1) defined a new set of syntax and opsem for symbolic exe. This syntax devides blocks into subblocks which are separated by 'call's. The simple symbolic execution does not cross calls and branching instructions. The opsem is of big-step style. We will prove that it is consistent with det-bigstep for LLVM.
2) proving that the symbolic execution results denotes the relations
between states before and after this opsem.

3) defined modules for LLVM's syntax and symbolic execution's syntax,
such that we can reuse names.

4) moved definitions about GenericValues into genericvalues.v

5) fixed bugs in LLVM's opsem.



git-svn-id: https://webdav.seas.upenn.edu/svn/sol/vol@2522 eef5ea85-cc2e-0410-bd84-0fae1f012da8

src/TV/symexe.v
@@ -9,7 +9,334 @@ Require Import monad.
 Require Import Arith.
 Require Import Metatheory.
 Require Import ssa_mem.
+Require Import genericvalues.
 Require Import ssa_dynamic.
+Require Import trace.
+
+(* Syntax easy to be proved with symbolic execution. *)
+
+Module SimpleSE.
+
+Inductive cmd : Set := 
+ | insn_bop : id -> bop -> sz -> value -> value -> cmd
+ | insn_extractvalue : id -> typ -> value -> list const -> cmd
+ | insn_insertvalue : id -> typ -> value -> typ -> value -> list const -> cmd
+ | insn_malloc : id -> typ -> sz -> align -> cmd
+ | insn_free : id -> typ -> value -> cmd
+ | insn_alloca : id -> typ -> sz -> align -> cmd
+ | insn_load : id -> typ -> value -> cmd
+ | insn_store : id -> typ -> value -> value -> cmd
+ | insn_gep : id -> inbounds -> typ -> value -> list value -> cmd
+ | insn_ext : id -> extop -> typ -> value -> typ -> cmd
+ | insn_cast : id -> castop -> typ -> value -> typ -> cmd
+ | insn_icmp : id -> cond -> typ -> value -> value -> cmd
+ | insn_select : id -> value -> typ -> value -> value -> cmd
+.
+
+Tactic Notation "cmd_cases" tactic(first) tactic(c) :=
+  first;
+  [ c "insn_bop" | c "insn_extractvalue" | c "insn_insertvalue" |
+    c "insn_malloc" | c "insn_free" |
+    c "insn_alloca" | c "insn_load" | c "insn_store" | c "insn_gep" |
+    c "insn_ext" | c "insn_cast" | c "insn_icmp" |  c "insn_select" ].
+
+Inductive call : Set := 
+ | insn_call : id -> noret -> tailc -> typ -> id -> list_param -> call.
+
+Inductive subblock : Set :=
+ | subblock_intro : list cmd -> call -> subblock.
+
+Inductive block : Set :=
+ | block_intro : l -> list phinode -> list subblock -> terminator -> block.
+
+Inductive fdef : Set := 
+ | fdef_intro : fheader -> list block -> fdef.
+
+Inductive product : Set := 
+ | product_gvar : gvar -> product
+ | product_fdec : fdec -> product
+ | product_fdef : fdef -> product.
+
+Inductive module : Set := 
+ | module_intro : list_layout -> list product -> module.
+
+Definition system : Set := list module.
+
+(***************************************************************)
+
+Record ExecutionContext : Set := mkEC {
+CurFunction : fdef;
+CurBB       : block;
+CurCmds     : list subblock;         (* subblock to run within CurBB *)
+Terminator  : terminator;
+Locals      : GVMap;                 (* LLVM values used in this invocation *)
+Args        : list GenericValue;      
+Allocas     : list mblock            (* Track memory allocated by alloca *)
+}.
+
+Definition ECStack := list ExecutionContext.
+
+Record State : Set := mkState {
+CurSystem      : system;
+CurTatgetData  : layouts;
+CurProducts    : list product;
+ECS            : ECStack;
+Globals        : GVMap;
+Mem            : mem
+}.
+
+(* deterministic big-step for this new syntax with subblocks. *)
+
+Variable lookupBlockViaLabelFromSystem : system -> l -> option block.
+Variable switchToNewBasicBlock : block -> block -> GVMap -> GVMap.
+Variable lookupFdefViaIDFromSystem : system -> id -> option fdef.
+Variable getEntryBlock : fdef -> option block.
+
+Inductive dbCmd : State -> State -> trace -> Prop :=
+| dbBop: forall S TD Ps F B lc gl lc' gl' arg id bop sz v1 v2 gv3 EC cs c sbs tmn Mem als,
+  BOP TD lc gl bop sz v1 v2 = Some gv3 ->
+  updateEnv lc gl id gv3 = (lc', gl') -> 
+  dbCmd 
+    (mkState S TD Ps ((mkEC F B ((subblock_intro ((insn_bop id bop sz v1 v2)::cs) c)::sbs) tmn lc arg als)::EC) gl Mem) 
+    (mkState S TD Ps ((mkEC F B ((subblock_intro cs c)::sbs) tmn lc' arg als)::EC) gl' Mem)
+    trace_nil 
+| dbExtractValue : forall S TD Ps F B lc gl lc' gl' arg id t v gv gv' idxs EC cs c sbs tmn Mem als,
+  getOperandValue TD v lc gl = Some gv ->
+  extractGenericValue TD t gv idxs = Some gv' ->
+  updateEnv lc gl id gv' = (lc', gl') -> 
+  dbCmd 
+    (mkState S TD Ps ((mkEC F B ((subblock_intro ((insn_extractvalue id t v idxs)::cs) c)::sbs) tmn lc arg als)::EC) gl Mem) 
+    (mkState S TD Ps ((mkEC F B ((subblock_intro cs c)::sbs) tmn lc' arg als)::EC) gl' Mem)
+    trace_nil 
+| dbInsertValue : forall S TD Ps F B lc gl lc' gl' arg id t v t' v' gv gv' gv'' idxs EC cs c sbs tmn Mem als,
+  getOperandValue TD v lc gl = Some gv ->
+  getOperandValue TD v' lc gl = Some gv' ->
+  insertGenericValue TD t gv idxs t' gv' = Some gv'' ->
+  updateEnv lc gl id gv'' = (lc', gl') -> 
+  dbCmd 
+    (mkState S TD Ps ((mkEC F B ((subblock_intro ((insn_insertvalue id t v t' v' idxs)::cs) c)::sbs) tmn lc arg als)::EC) gl Mem) 
+    (mkState S TD Ps ((mkEC F B ((subblock_intro cs c)::sbs) tmn lc' arg als)::EC) gl' Mem)
+    trace_nil 
+| dbMalloc : forall S TD Ps F B lc gl lc' gl' arg id t sz align EC cs c sbs tmn Mem als Mem' tsz mb,
+  getTypeAllocSize TD t = Some tsz ->
+  malloc TD Mem (tsz * sz) align = Some (Mem', mb) ->
+  updateEnv lc gl id (ptr2GV TD (mb, 0)) = (lc', gl') -> 
+  dbCmd 
+    (mkState S TD Ps ((mkEC F B ((subblock_intro ((insn_malloc id t sz align)::cs) c)::sbs) tmn lc arg als)::EC) gl Mem) 
+    (mkState S TD Ps ((mkEC F B ((subblock_intro cs c)::sbs) tmn lc' arg als)::EC) gl' Mem')
+    trace_nil
+| dbFree : forall S TD Ps F B lc gl arg fid t v EC cs c sbs tmn Mem als Mem' mptr,
+  getOperandPtr TD v lc gl = Some mptr ->
+  free Mem mptr = Some Mem'->
+  dbCmd 
+    (mkState S TD Ps ((mkEC F B ((subblock_intro ((insn_free fid t v)::cs) c)::sbs) tmn lc arg als)::EC) gl Mem) 
+    (mkState S TD Ps ((mkEC F B ((subblock_intro cs c)::sbs) tmn lc arg als)::EC) gl Mem')
+    trace_nil
+| dbAlloca : forall S TD Ps F B lc gl lc' gl' arg id t sz align EC cs c sbs tmn Mem als Mem' tsz mb,
+  getTypeAllocSize TD t = Some tsz ->
+  malloc TD Mem (tsz * sz) align = Some (Mem', mb) ->
+  updateEnv lc gl id (ptr2GV TD (mb, 0)) = (lc', gl') -> 
+  dbCmd 
+    (mkState S TD Ps ((mkEC F B ((subblock_intro ((insn_alloca id t sz align)::cs) c)::sbs) tmn lc arg als)::EC) gl Mem) 
+    (mkState S TD Ps ((mkEC F B ((subblock_intro cs c)::sbs) tmn lc' arg (mb::als))::EC) gl' Mem')
+    trace_nil
+| dbLoad : forall S TD Ps F B lc gl lc' gl' arg id t v EC cs c sbs tmn Mem als mp gv,
+  getOperandPtr TD v lc gl = Some mp ->
+  mload TD Mem mp t = Some gv ->
+  updateEnv lc gl id gv = (lc', gl') -> 
+  dbCmd 
+    (mkState S TD Ps ((mkEC F B ((subblock_intro ((insn_load id t v)::cs) c)::sbs) tmn lc arg als)::EC) gl Mem) 
+    (mkState S TD Ps ((mkEC F B ((subblock_intro cs c)::sbs) tmn lc' arg als)::EC) gl' Mem)
+    trace_nil
+| dbStore : forall S TD Ps F B lc gl arg sid t v1 v2 EC cs c sbs tmn Mem als mp2 gv1 Mem',
+  getOperandValue TD v1 lc gl = Some gv1 ->
+  getOperandPtr TD v2 lc gl = Some mp2 ->
+  mstore TD Mem mp2 t gv1 = Some Mem' ->
+  dbCmd 
+    (mkState S TD Ps ((mkEC F B ((subblock_intro ((insn_store sid t v1 v2)::cs) c)::sbs) tmn lc arg als)::EC) gl Mem) 
+    (mkState S TD Ps ((mkEC F B ((subblock_intro cs c)::sbs) tmn lc arg als)::EC) gl Mem')
+    trace_nil
+| dbGEP : forall S TD Ps F B lc gl lc' gl' arg id inbounds t v idxs EC mp mp' cs c sbs tmn Mem als,
+  getOperandPtr TD v lc gl = Some mp ->
+  GEP TD lc gl t mp idxs inbounds = Some mp' ->
+  updateEnv lc gl id (ptr2GV TD mp') = (lc', gl') -> 
+  dbCmd 
+    (mkState S TD Ps ((mkEC F B ((subblock_intro ((insn_gep id inbounds t v idxs)::cs) c)::sbs) tmn lc arg als)::EC) gl Mem) 
+    (mkState S TD Ps ((mkEC F B ((subblock_intro cs c)::sbs) tmn lc' arg als)::EC) gl' Mem)
+    trace_nil 
+| dbExt : forall S TD Ps F B lc gl arg id extop t1 v1 t2 gv2 EC cs c sbs tmn lc' gl' Mem als,
+  EXT TD lc gl extop t1 v1 t2 = Some gv2 ->
+  updateEnv lc gl id gv2 = (lc', gl') -> 
+  dbCmd 
+    (mkState S TD Ps ((mkEC F B ((subblock_intro ((insn_ext id extop t1 v1 t2)::cs) c)::sbs) tmn lc arg als)::EC) gl Mem) 
+    (mkState S TD Ps ((mkEC F B ((subblock_intro cs c)::sbs) tmn lc' arg als)::EC) gl' Mem)
+    trace_nil
+| dbCast : forall S TD Ps F B lc gl arg id castop t1 v1 t2 gv2 EC cs c sbs tmn lc' gl' Mem als,
+  CAST TD lc gl castop t1 v1 t2 = Some gv2 ->
+  updateEnv lc gl id gv2 = (lc', gl') -> 
+  dbCmd 
+    (mkState S TD Ps ((mkEC F B ((subblock_intro ((insn_cast id castop t1 v1 t2)::cs) c)::sbs) tmn lc arg als)::EC) gl Mem) 
+    (mkState S TD Ps ((mkEC F B ((subblock_intro cs c)::sbs) tmn lc' arg als)::EC) gl' Mem)
+    trace_nil
+| dbIcmp : forall S TD Ps F B lc gl arg id cond t v1 v2 gv3 EC cs c sbs tmn lc' gl' Mem als,
+  ICMP TD lc gl cond t v1 v2 = Some gv3 ->
+  updateEnv lc gl id gv3 = (lc', gl') -> 
+  dbCmd 
+    (mkState S TD Ps ((mkEC F B ((subblock_intro ((insn_icmp id cond t v1 v2)::cs) c)::sbs) tmn lc arg als)::EC) gl Mem) 
+    (mkState S TD Ps ((mkEC F B ((subblock_intro cs c)::sbs) tmn lc' arg als)::EC) gl' Mem)
+    trace_nil
+| dbSelect : forall S TD Ps F B lc gl arg id v0 t v1 v2 cond EC cs c sbs tmn lc' gl' Mem als gv1 gv2,
+  getOperandInt TD 1 v0 lc gl = Some cond ->
+  getOperandValue TD v1 lc gl = Some gv1 ->
+  getOperandValue TD v2 lc gl = Some gv2 ->
+  (lc', gl') = (if cond
+               then updateEnv lc gl id gv1
+               else updateEnv lc gl id gv2) ->
+  dbCmd 
+    (mkState S TD Ps ((mkEC F B ((subblock_intro ((insn_select id v0 t v1 v2)::cs) c)::sbs) tmn lc arg als)::EC) gl Mem) 
+    (mkState S TD Ps ((mkEC F B ((subblock_intro cs c)::sbs) tmn lc' arg als)::EC) gl' Mem)
+    trace_nil
+.
+
+Inductive dbTerminator : State -> State -> trace -> Prop :=
+| dbBranch : forall S TD Ps F B lc gl arg bid Cond l1 l2 c
+                              l' ps' sbs' tmn' lc' EC Mem als,   
+  getOperandInt TD 1 Cond lc gl = Some c ->
+  Some (block_intro l' ps' sbs' tmn') = (if c 
+               then lookupBlockViaLabelFromSystem S l1
+               else lookupBlockViaLabelFromSystem S l2) ->
+  lc' = switchToNewBasicBlock (block_intro l' ps' sbs' tmn') B lc ->
+  dbTerminator 
+    (mkState S TD Ps ((mkEC F B nil (insn_br bid Cond l1 l2) lc arg als)::EC) gl Mem)
+    (mkState S TD Ps ((mkEC F (block_intro l' ps' sbs' tmn') sbs' tmn' lc' arg als)::EC) gl Mem)
+    trace_nil 
+| dbBranch_uncond : forall S TD Ps F B lc gl arg l bid
+                              l' ps' sbs' tmn' lc' EC Mem als,   
+  Some (block_intro l' ps' sbs' tmn') = (lookupBlockViaLabelFromSystem S l) ->
+  lc' = switchToNewBasicBlock (block_intro l' ps' sbs' tmn') B lc ->
+  dbTerminator 
+    (mkState S TD Ps ((mkEC F B nil (insn_br_uncond bid l) lc arg als)::EC) gl Mem)
+    (mkState S TD Ps ((mkEC F (block_intro l' ps' sbs' tmn') sbs' tmn' lc' arg als)::EC) gl Mem)
+    trace_nil 
+.
+
+Inductive dbCmds : State -> State -> trace -> Prop :=
+| dbCmds_nil : forall S, dbCmds S S trace_nil
+| dbCmds_cons : forall S1 S2 S3 t1 t2,
+    dbCmd S1 S2 t1 ->
+    dbCmds S2 S3 t2 ->
+    dbCmds S1 S3 (trace_app t1 t2).
+
+Inductive dbCall : State -> State -> trace -> Prop :=
+| dbCall_intro : forall S TD Ps F B lc gl arg rid noret tailc rt fid lp gl' gl'' sbs tmn
+                       EC Rid oResult tr lc'' B' lc' Mem Mem' als' als Mem'',
+  dbFdef fid rt lp S TD Ps ((mkEC F B ((subblock_intro nil (insn_call rid noret tailc rt fid lp))::sbs) tmn lc arg als)::EC) lc gl Mem lc' gl' als' Mem' B' Rid oResult tr ->
+  (lc'', gl'') = 
+    match noret with
+    | false =>
+      if (LLVMlib.typEqB rt typ_void) 
+      then (lc, gl') 
+      else 
+        match oResult with
+        | None => (lc, gl')
+        | Some Result => 
+          match (getOperandValue TD Result lc' gl') with
+          | Some gr => updateEnv lc gl' rid gr
+          | None => (lc, gl')
+          end
+        end
+    | true => (lc, gl')
+    end ->
+  free_allocas Mem' als' = Some Mem'' ->
+  dbCall 
+    (mkState S TD Ps ((mkEC F B ((subblock_intro nil (insn_call rid noret tailc rt fid lp))::sbs) tmn lc arg als)::EC) gl Mem) 
+    (mkState S TD Ps ((mkEC F B sbs tmn lc'' arg als)::EC) gl'' Mem'') 
+    tr
+with dbSubblock : State -> State -> trace -> Prop :=
+| dbSubblock_intro : forall state1 state2 tr1 state3 tr2,
+  dbCmds state1 state2 tr1 ->
+  dbCall state2 state3 tr2 ->
+  dbSubblock state1 state3 (trace_app tr1 tr2)
+with dbSubblocks : State -> State -> trace -> Prop :=
+| dbSubblocks_nil : forall S, dbSubblocks S S trace_nil
+| dbSubblocks_cond : forall S1 S2 S3 t1 t2,
+    dbSubblock S1 S2 t1 ->
+    dbSubblocks S2 S3 t2 ->
+    dbSubblocks S1 S3 (trace_app t1 t2)
+with dbBlock : State -> State -> trace -> Prop :=
+| dbBlock_intro : forall state1 state2 tr1 state3 tr2,
+  dbSubblocks state1 state2 tr1 ->
+  dbTerminator state2 state3 tr2 ->
+  dbBlock state1 state3 (trace_app tr1 tr2)
+with dbBlocks : State -> State -> trace -> Prop :=
+| dbBlocks_nil : forall S, dbBlocks S S trace_nil
+| dbBlocks_cons : forall S1 S2 S3 t1 t2,
+    dbBlock S1 S2 t1 ->
+    dbBlocks S2 S3 t2 ->
+    dbBlocks S1 S3 (trace_app t1 t2)
+with dbFdef : id -> typ -> list_param -> system -> layouts -> list product -> list ExecutionContext -> GVMap -> GVMap -> mem -> GVMap -> GVMap -> list mblock -> mem -> block -> id -> option value -> trace -> Prop :=
+| dbFdef_func : forall S TD Ps gl fid lp lc rid
+                            l' ps' cs' tmn' rt la lb B'' Result lc' gl' tr ECs Mem Mem' als',
+  lookupFdefViaIDFromSystem S fid = Some (fdef_intro (fheader_intro rt fid la) lb) ->
+  getEntryBlock (fdef_intro (fheader_intro rt fid la) lb) = Some (block_intro l' ps' cs' tmn') ->
+  dbBlocks 
+    (mkState S TD Ps ((mkEC (fdef_intro (fheader_intro rt fid la) lb) 
+                             (block_intro l' ps' cs' tmn') cs' tmn' (initLocals la (params2GVs TD lp lc gl))
+                            (params2GVs TD lp lc gl) nil)::ECs) gl Mem)
+    (mkState S TD Ps ((mkEC (fdef_intro (fheader_intro rt fid la) lb) 
+                             B'' nil (insn_return rid rt Result) lc'
+                            (params2GVs TD lp lc gl) als')::ECs) gl' Mem')
+    tr ->
+  dbFdef fid rt lp S TD Ps ECs lc gl Mem lc' gl' als' Mem' B'' rid (Some Result) tr
+| dbFdef_proc : forall S TD Ps gl fid lp lc rid
+                            l' ps' cs' tmn' rt la lb B'' lc' gl' tr ECs Mem Mem' als',
+  lookupFdefViaIDFromSystem S fid = Some (fdef_intro (fheader_intro rt fid la) lb) ->
+  getEntryBlock (fdef_intro (fheader_intro rt fid la) lb) = Some (block_intro l' ps' cs' tmn') ->
+  dbBlocks 
+    (mkState S TD Ps ((mkEC (fdef_intro (fheader_intro rt fid la) lb) 
+                             (block_intro l' ps' cs' tmn') cs' tmn' (initLocals la (params2GVs TD lp lc gl))
+                            (params2GVs TD lp lc gl) nil)::ECs) gl Mem)
+    (mkState S TD Ps ((mkEC (fdef_intro (fheader_intro rt fid la) lb) 
+                             B'' nil (insn_return_void rid) lc'
+                            (params2GVs TD lp lc gl) als')::ECs) gl' Mem')
+    tr ->
+  dbFdef fid  rt lp S TD Ps ECs lc gl Mem lc' gl' als' Mem' B'' rid None tr
+.
+
+Scheme dbCall_ind2 := Induction for dbCall Sort Prop
+  with dbSubblock_ind2 := Induction for dbSubblock Sort Prop
+  with dbSubblocks_ind2 := Induction for dbSubblocks Sort Prop
+  with dbBlock_ind2 := Induction for dbBlock Sort Prop
+  with dbBlocks_ind2 := Induction for dbBlocks Sort Prop
+  with dbFdef_ind2 := Induction for dbFdef Sort Prop.
+
+Combined Scheme db_mutind from dbCall_ind2, dbSubblock_ind2, dbSubblocks_ind2,
+                               dbBlock_ind2, dbBlocks_ind2, dbFdef_ind2.
+
+Tactic Notation "db_mutind_cases" tactic(first) tactic(c) :=
+  first;
+  [ c "dbCall_intro" | 
+    c "dbSubblock_intro" | c "dbSubblocks_nil" | c "dbSubblocks_cons" | 
+    c "dbBlock_intro" | c "dbBlocks_nil" | c "dbBlocks_cons" | 
+    c "dbFdef_func" | c "dbFdef_proc" ].
+
+Tactic Notation "dbCmd_cases" tactic(first) tactic(c) :=
+  first;
+  [ c "dbBop" | c "dbExtractValue" | c "dbInsertValue" |
+    c "dbMalloc" | c "dbFree" |
+    c "dbAlloca" | c "dbLoad" | c "dbStore" | c "dbGEP" |
+    c "dbExt" | c "dbCast" | c "dbIcmp" |  c "dbSelect" ].
+
+Tactic Notation "dbTerminator_cases" tactic(first) tactic(c) :=
+  first;
+  [ c "dbBranch" | c "dbBranch_uncond" ].
+
+Tactic Notation "dbCmds_cases" tactic(first) tactic(c) :=
+  first;
+  [ c "dbCmds_nil" | c "dbCmds_cons" ].
+
+Hint Constructors dbCmd dbCmds dbTerminator dbCall 
+                  dbSubblock dbSubblocks dbBlock dbBlocks dbFdef.
 
 (** symbolic terms and memories. *)
 Inductive sterm : Set := 
@@ -26,7 +353,6 @@ Inductive sterm : Set :=
 | sterm_icmp : cond -> typ -> sterm -> sterm -> sterm
 | sterm_phi : typ -> list (sterm*l) -> sterm
 | sterm_select : sterm -> typ -> sterm -> sterm -> sterm
-| sterm_call : noret -> tailc -> typ -> id -> list (typ*sterm) -> sterm
 with smem : Set :=
 | smem_init : smem
 | smem_malloc : smem -> typ -> sz -> align -> smem
@@ -37,21 +363,23 @@ with smem : Set :=
 .
 
 Inductive sterminator : Set :=
-| stmn_return : typ -> sterm -> sterminator
-| stmn_return_void : sterminator
-| stmn_br : sterm -> l -> l -> sterminator
-| stmn_br_uncond : l -> sterminator
-| stmn_unreachable : sterminator
+| stmn_return : id -> typ -> sterm -> sterminator
+| stmn_return_void : id -> sterminator
+| stmn_br : id -> sterm -> l -> l -> sterminator
+| stmn_br_uncond : id -> l -> sterminator
+| stmn_unreachable : id -> sterminator
+.
+
+Inductive scall : Set :=
+| stmn_call : id -> noret -> tailc -> typ -> id -> list (typ*sterm) -> scall
 .
 
 Definition smap := list (atom*sterm).
-Definition effects := list sterm.
 
 Record sstate : Set := mkSstate 
 {
   STerms : smap;
-  SMem : smem;
-  Effects : effects
+  SMem : smem
 }.
 
 Fixpoint updateSmap (sm:smap) (id0:id) (s0:sterm) : smap :=
@@ -96,14 +424,6 @@ match s with
                    lsl1)
 | sterm_select s1 t1 s2 s3 => 
     sterm_select (subst_tt id0 s0 s1) t1 (subst_tt id0 s0 s2) (subst_tt id0 s0 s3)
-| sterm_call noret tailc t1 id1 lts1 => 
-    sterm_call noret tailc t1 id1 
-                 (List.map 
-                   (fun (ts1:typ*sterm) => 
-                    let (t1,s1):=ts1 in 
-                    (t1, (subst_tt id0 s0 s1))
-                   ) 
-                   lts1)
 end
 with subst_tm (id0:id) (s0:sterm) (m:smem) : smem :=
 match m with 
@@ -141,15 +461,13 @@ match i with
                    (sterm_bop op0 sz0 
                      (subst_mt st.(STerms) (sterm_val v1))
                      (subst_mt st.(STerms) (sterm_val v2))))
-                 st.(SMem)
-                 st.(Effects))
+                 st.(SMem))
 | insn_extractvalue id0 t1 v1 cs3 =>
        (mkSstate (updateSmap st.(STerms) id0 
                    (sterm_extractvalue t1 
                      (subst_mt st.(STerms) (sterm_val v1))
                      cs3))
-                 st.(SMem) 
-                 st.(Effects))
+                 st.(SMem))
 | insn_insertvalue id0 t1 v1 t2 v2 cs3 =>  
        (mkSstate (updateSmap st.(STerms) id0 
                    (sterm_insertvalue 
@@ -158,8 +476,7 @@ match i with
                      t2 
                      (subst_mt st.(STerms) (sterm_val v2))
                      cs3))
-                 st.(SMem) 
-                 st.(Effects))
+                 st.(SMem))
 | insn_malloc id0 t1 sz1 al1 =>  
        (mkSstate (updateSmap st.(STerms) id0 
                    (sterm_malloc 
@@ -167,20 +484,17 @@ match i with
                      t1 sz1 al1))
                  (smem_malloc 
                    (subst_mm st.(STerms) st.(SMem)) 
-                   t1 sz1 al1)
-                 st.(Effects))
+                   t1 sz1 al1))
 | insn_free id0 t0 v0 =>  
        (mkSstate st.(STerms)
                 (smem_free st.(SMem) t0 
-                  (subst_mt st.(STerms) (sterm_val v0)))
-                 st.(Effects))
+                  (subst_mt st.(STerms) (sterm_val v0))))
 | insn_alloca id0 t1 sz1 al1 =>  
        (mkSstate (updateSmap st.(STerms) id0 
                    (sterm_alloca 
                      (subst_mm st.(STerms) st.(SMem)) t1 sz1 al1))
                  (smem_alloca 
-                   (subst_mm st.(STerms) st.(SMem)) t1 sz1 al1)
-                 st.(Effects))
+                   (subst_mm st.(STerms) st.(SMem)) t1 sz1 al1))
 | insn_load id0 t2 v2 =>  
        (mkSstate (updateSmap st.(STerms) id0 
                    (sterm_load 
@@ -190,44 +504,38 @@ match i with
                  (smem_load 
                    (subst_mm st.(STerms) st.(SMem))
                    t2 
-                   (subst_mt st.(STerms) (sterm_val v2)))
-                 st.(Effects))
+                   (subst_mt st.(STerms) (sterm_val v2))))
 | insn_store id0 t0 v1 v2 =>  
        (mkSstate st.(STerms)
                  (smem_store 
                    (subst_mm st.(STerms) st.(SMem))
                    t0 
                    (subst_mt st.(STerms) (sterm_val v1))
-                   (subst_mt st.(STerms) (sterm_val v2)))
-                 st.(Effects))
+                   (subst_mt st.(STerms) (sterm_val v2))))
 | insn_gep id0 inbounds0 t1 v1 lv2 =>  
        (mkSstate (updateSmap st.(STerms) id0 
                    (sterm_gep inbounds0 t1 
                      (subst_mt st.(STerms) (sterm_val v1))
                      (List.map (subst_mt st.(STerms)) (List.map sterm_val lv2))))
-                 st.(SMem) 
-                 st.(Effects))
+                 st.(SMem))
 | insn_ext id0 op0 t1 v1 t2 =>  
        (mkSstate (updateSmap st.(STerms) id0 
                    (sterm_ext op0 t1 
                      (subst_mt st.(STerms) (sterm_val v1))
                      t2))
-                 st.(SMem) 
-                 st.(Effects))
+                 st.(SMem))
 | insn_cast id0 op0 t1 v1 t2 =>  
        (mkSstate (updateSmap st.(STerms) id0 
                    (sterm_cast op0 t1 
                      (subst_mt st.(STerms) (sterm_val v1))
                      t2))
-                 st.(SMem) 
-                 st.(Effects))
+                 st.(SMem))
 | insn_icmp id0 c0 t0 v1 v2 =>  
        (mkSstate (updateSmap st.(STerms) id0 
                    (sterm_icmp c0 t0 
                      (subst_mt st.(STerms) (sterm_val v1))
                      (subst_mt st.(STerms) (sterm_val v2))))
-                 st.(SMem) 
-                 st.(Effects))
+                 st.(SMem))
 | insn_select id0 v0 t0 v1 v2 =>  
        (mkSstate (updateSmap st.(STerms) id0 
                    (sterm_select 
@@ -235,20 +543,9 @@ match i with
                      t0 
                      (subst_mt st.(STerms) (sterm_val v1))
                      (subst_mt st.(STerms) (sterm_val v2))))
-                 st.(SMem) 
-                 st.(Effects))
-| insn_call id0 false tailc0 t1 id1 list_param1 =>  
-       (mkSstate (updateSmap st.(STerms) id0 
-                   (sterm_call false tailc0 t1 id1 
-                      (list_param__list_typ_subst_sterm list_param1 st.(STerms))))
-                 st.(SMem) 
-                 st.(Effects))
-| insn_call id0 true tailc0 t1 id1 list_param1 =>  
-       (mkSstate st.(STerms)
-                 st.(SMem) 
-                 ((sterm_call true tailc0 t1 id1 
-                    (list_param__list_typ_subst_sterm list_param1 st.(STerms)))::st.(Effects)))
+                 st.(SMem))
 end.
+
 
 Fixpoint _se_phinodes (st st0: sstate) (ps:list phinode) : sstate :=
 match ps with
@@ -267,8 +564,7 @@ match ps with
                    )
                  )
                )
-               st.(SMem)
-               st.(Effects))
+               st.(SMem))
      st0
      ps'
 end.
@@ -283,37 +579,18 @@ end.
 
 Definition se_terminator (st : sstate) (i:terminator) : sterminator :=
 match i with 
-| insn_return id0 t0 v0 => stmn_return t0 (subst_mt st.(STerms) (sterm_val v0))
-| insn_return_void id0 => stmn_return_void
-| insn_br id0 v0 l1 l2 => stmn_br (subst_mt st.(STerms) (sterm_val v0)) l1 l2
-| insn_br_uncond id0 l0 => stmn_br_uncond l0
-| insn_unreachable id0 => stmn_unreachable
+| insn_return id0 t0 v0 => stmn_return id0 t0 (subst_mt st.(STerms) (sterm_val v0))
+| insn_return_void id0 => stmn_return_void id0 
+| insn_br id0 v0 l1 l2 => stmn_br id0 (subst_mt st.(STerms) (sterm_val v0)) l1 l2
+| insn_br_uncond id0 l0 => stmn_br_uncond id0 l0
+| insn_unreachable id0 => stmn_unreachable id0 
 end.
 
-Definition se_block (st : sstate) (b:block) : sstate*sterminator :=
-match b with
-| block_intro l0 ps cs tmn =>
-  let st0 := se_cmds (se_phinodes st ps) cs in
-  (st0, se_terminator st0 tmn)
-end.
-
-Definition tv_block (b1 b2:block) :=
-let (st1, tmn1) := se_block (mkSstate nil smem_init nil) b1 in
-let (st2, tmn2) := se_block (mkSstate nil smem_init nil) b2 in
-st1 = st2 /\ tmn1 = tmn2.
-
-Fixpoint GVs2Nats (TD:layouts) (lgv:list GenericValue) (locals:GVMap) (globals:GVMap) : option (list nat):=
-match lgv with
-| nil => Some nil
-| gv::lgv' => 
-    match (GV2nat TD 32 gv) with
-    | Some n =>
-      match (GVs2Nats TD lgv' locals globals) with
-      | Some ns => Some (n::ns)
-      | None => None
-      end
-    | None => None
-    end
+Definition se_call (st : sstate) (i:call) : scall :=
+match i with
+| insn_call id0 noret tailc0 t1 id1 list_param1 =>  
+                   (stmn_call id0 noret tailc0 t1 id1 
+                      (list_param__list_typ_subst_sterm list_param1 st.(STerms)))
 end.
 
 Inductive sterm_denotes_genericvalue : 
@@ -325,7 +602,7 @@ Inductive sterm_denotes_genericvalue :
    GenericValue ->          (* value that denotes sterm *)
    Prop :=
 | sterm_val_denotes : forall TD lc gl Mem v gv,
-  getOperandValue TD v lc gl = Some gv ->
+  getOperandValue TD v lc gl = Some gv ->  
   sterm_denotes_genericvalue TD lc gl Mem (sterm_val v) gv
 | sterm_bop_denotes : forall TD lc gl Mem op0 sz0 st1 st2 gv1 gv2 gv3,
   sterm_denotes_genericvalue TD lc gl Mem st1 gv1 ->
@@ -334,26 +611,29 @@ Inductive sterm_denotes_genericvalue :
   sterm_denotes_genericvalue TD lc gl Mem (sterm_bop op0 sz0 st1 st2) gv3
 | sterm_extractvalue_denotes : forall TD lc gl Mem t1 st1 idxs0 gv1 gv2,
   sterm_denotes_genericvalue TD lc gl Mem st1 gv1 ->
-  extractGenericValue TD lc gl t1 gv1 idxs0 = Some gv2 ->
+  extractGenericValue TD t1 gv1 idxs0 = Some gv2 ->
   sterm_denotes_genericvalue TD lc gl Mem (sterm_extractvalue t1 st1 idxs0) gv2
 | sterm_insertvalue_denotes : forall TD lc gl Mem t1 st1 t2 st2 idxs0 gv1 gv2 gv3,
   sterm_denotes_genericvalue TD lc gl Mem st1 gv1 ->
   sterm_denotes_genericvalue TD lc gl Mem st2 gv2 ->
-  insertGenericValue TD t1 gv1 lc gl idxs0 t2 gv2 = Some gv3 ->
+  insertGenericValue TD t1 gv1 idxs0 t2 gv2 = Some gv3 ->
   sterm_denotes_genericvalue TD lc gl Mem (sterm_insertvalue t1 st1 t2 st2 idxs0) gv3
-| sterm_malloc_denotes : forall TD lc gl Mem sm0 t0 sz0 align0 tsz0 Mem' mb,
+| sterm_malloc_denotes : forall TD lc gl Mem0 Mem1 sm0 t0 sz0 align0 tsz0 Mem2 mb,
+  smem_denotes_mem TD lc gl Mem0 sm0 Mem1 ->
   getTypeAllocSize TD t0 = Some tsz0 ->
-  malloc TD Mem (tsz0 * sz0) align0 = Some (Mem', mb) ->
-  sterm_denotes_genericvalue TD lc gl Mem (sterm_malloc sm0 t0 sz0 align0) (ptr2GV TD (mb, 0))
-| sterm_alloca_denotes : forall TD lc gl Mem sm0 t0 sz0 align0 tsz0 Mem' mb,
+  malloc TD Mem1 (tsz0 * sz0) align0 = Some (Mem2, mb) ->
+  sterm_denotes_genericvalue TD lc gl Mem0 (sterm_malloc sm0 t0 sz0 align0) (ptr2GV TD (mb, 0))
+| sterm_alloca_denotes : forall TD lc gl Mem0 Mem1 sm0 t0 sz0 align0 tsz0 Mem2 mb,
+  smem_denotes_mem TD lc gl Mem0 sm0 Mem1 ->
   getTypeAllocSize TD t0 = Some tsz0 ->
-  malloc TD Mem (tsz0 * sz0) align0 = Some (Mem', mb) ->
-  sterm_denotes_genericvalue TD lc gl Mem (sterm_alloca sm0 t0 sz0 align0) (ptr2GV TD (mb, 0))
-| sterm_load_denotes : forall TD lc gl Mem sm0 t0 st0 gv0 mp0 gv1,
-  sterm_denotes_genericvalue TD lc gl Mem st0 gv0 ->
+  malloc TD Mem1 (tsz0 * sz0) align0 = Some (Mem2, mb) ->
+  sterm_denotes_genericvalue TD lc gl Mem0 (sterm_alloca sm0 t0 sz0 align0) (ptr2GV TD (mb, 0))
+| sterm_load_denotes : forall TD lc gl Mem0 Mem1 sm0 t0 st0 gv0 mp0 gv1,
+  sterm_denotes_genericvalue TD lc gl Mem0 st0 gv0 ->
+  smem_denotes_mem TD lc gl Mem0 sm0 Mem1 ->
   GV2ptr TD (getPointerSize TD) gv0 = Some mp0 ->
-  mload TD Mem mp0 t0 = Some gv1 ->
-  sterm_denotes_genericvalue TD lc gl Mem (sterm_load sm0 t0 st0) gv1
+  mload TD Mem1 mp0 t0 = Some gv1 ->
+  sterm_denotes_genericvalue TD lc gl Mem0 (sterm_load sm0 t0 st0) gv1
 | sterm_gep_denotes : forall TD lc gl Mem ib0 t0 st0 sts0 gv0 gvs0 ns0 mp0 mp1,
   sterm_denotes_genericvalue TD lc gl Mem st0 gv0 ->
   sterms_denote_genericvalues TD lc gl Mem sts0 gvs0 ->
@@ -374,12 +654,13 @@ Inductive sterm_denotes_genericvalue :
   sterm_denotes_genericvalue TD lc gl Mem st2 gv2 ->
   micmp TD cond0 t0 gv1 gv2 = Some gv3 ->
   sterm_denotes_genericvalue TD lc gl Mem (sterm_icmp cond0 t0 st1 st2) gv3
-| sterm_select_denotes : forall TD lc gl Mem st0 t0 st1 st2 gv0 gv1 gv2 c0,
+| sterm_select_denotes : forall TD lc gl Mem st0 t0 st1 st2 gv0 gv1 gv2 c0 gv3,
   sterm_denotes_genericvalue TD lc gl Mem st0 gv0 ->
   sterm_denotes_genericvalue TD lc gl Mem st1 gv1 ->
   sterm_denotes_genericvalue TD lc gl Mem st2 gv2 ->
   GV2nat TD 1 gv0 = Some c0 ->
-  sterm_denotes_genericvalue TD lc gl Mem (sterm_select st0 t0 st1 st2) (if c0 then gv1 else gv2)
+  (if c0 then gv1 else gv2) = gv3 -> 
+  sterm_denotes_genericvalue TD lc gl Mem (sterm_select st0 t0 st1 st2) gv3
 with sterms_denote_genericvalues : 
    layouts ->               (* CurTatgetData *)
    GVMap ->                 (* local registers *)
@@ -403,38 +684,911 @@ with smem_denotes_mem :
    mem ->                   (* value that denotes smem *)
    Prop :=
 | smem_init_denotes : forall TD lc gl Mem,
-  smem_denotes_mem TD lc gl Mem smem_init initmem
-| smem_malloc_denotes : forall TD lc gl Mem sm0 t0 sz0 align0 tsz0 Mem' mb,
+  smem_denotes_mem TD lc gl Mem smem_init Mem
+| smem_malloc_denotes : forall TD lc gl Mem0 Mem1 sm0 t0 sz0 align0 tsz0 Mem2 mb,
+  smem_denotes_mem TD lc gl Mem0 sm0 Mem1 ->
   getTypeAllocSize TD t0 = Some tsz0 ->
-  malloc TD Mem (tsz0 * sz0) align0 = Some (Mem', mb) ->
-  smem_denotes_mem TD lc gl Mem (smem_malloc sm0 t0 sz0 align0) Mem'
-| smem_free_denotes : forall TD lc gl Mem sm0 t0 st0 gv0 mptr0 Mem',
-  sterm_denotes_genericvalue TD lc gl Mem st0 gv0 ->
+  malloc TD Mem1 (tsz0 * sz0) align0 = Some (Mem2, mb) ->
+  smem_denotes_mem TD lc gl Mem0 (smem_malloc sm0 t0 sz0 align0) Mem2
+| smem_free_denotes : forall TD lc gl Mem0 Mem1 sm0 t0 st0 gv0 mptr0 Mem2,
+  sterm_denotes_genericvalue TD lc gl Mem0 st0 gv0 ->
+  smem_denotes_mem TD lc gl Mem0 sm0 Mem1 ->
   GV2ptr TD (getPointerSize TD) gv0 = Some mptr0 ->
-  free Mem mptr0 = Some Mem'->
-  smem_denotes_mem TD lc gl Mem (smem_free sm0 t0 st0) Mem'
-| smem_alloca_denotes : forall TD lc gl Mem sm0 t0 sz0 align0 tsz0 Mem' mb,
+  free Mem1 mptr0 = Some Mem2->
+  smem_denotes_mem TD lc gl Mem0 (smem_free sm0 t0 st0) Mem2
+| smem_alloca_denotes : forall TD lc gl Mem0 Mem1 sm0 t0 sz0 align0 tsz0 Mem2 mb,
+  smem_denotes_mem TD lc gl Mem0 sm0 Mem1 ->
   getTypeAllocSize TD t0 = Some tsz0 ->
-  malloc TD Mem (tsz0 * sz0) align0 = Some (Mem', mb) ->
-  smem_denotes_mem TD lc gl Mem (smem_alloca sm0 t0 sz0 align0) Mem
-| smem_load_denotes : forall TD lc gl Mem sm0 t0 st0 Mem0,
-  smem_denotes_mem TD lc gl Mem sm0 Mem0 ->
-  smem_denotes_mem TD lc gl Mem (smem_load sm0 t0 st0) Mem0
-| smem_store_denotes : forall TD lc gl Mem sm0 t0 st1 st2 gv1 gv2 mptr2 Mem',
-  sterm_denotes_genericvalue TD lc gl Mem st1 gv1 ->
-  sterm_denotes_genericvalue TD lc gl Mem st2 gv2 ->
+  malloc TD Mem1 (tsz0 * sz0) align0 = Some (Mem2, mb) ->
+  smem_denotes_mem TD lc gl Mem0 (smem_alloca sm0 t0 sz0 align0) Mem2
+| smem_load_denotes : forall TD lc gl Mem0 sm0 t0 st0 Mem1,
+  smem_denotes_mem TD lc gl Mem0 sm0 Mem1 ->
+  smem_denotes_mem TD lc gl Mem0 (smem_load sm0 t0 st0) Mem1
+| smem_store_denotes : forall TD lc gl Mem0 Mem1 sm0 t0 st1 st2 gv1 gv2 mptr2 Mem2,
+  sterm_denotes_genericvalue TD lc gl Mem0 st1 gv1 ->
+  sterm_denotes_genericvalue TD lc gl Mem0 st2 gv2 ->
+  smem_denotes_mem TD lc gl Mem0 sm0 Mem1 ->
   GV2ptr TD (getPointerSize TD) gv2 = Some mptr2 ->
-  mstore TD Mem mptr2 t0 gv1 = Some Mem' ->
-  smem_denotes_mem TD lc gl Mem (smem_store sm0 t0 st1 st2) Mem'
+  mstore TD Mem1 mptr2 t0 gv1 = Some Mem2 ->
+  smem_denotes_mem TD lc gl Mem0 (smem_store sm0 t0 st1 st2) Mem2
 .
 
-Definition sstate_denotes_state TD lc gl Mem sstate0 lc' gl' mem' :=
-(forall id0 st0 gv',  
-  binds id0 st0 sstate0.(STerms) ->
-  lookupEnv TD id0 lc' gl' = Some gv' ->
-  sterm_denotes_genericvalue TD lc gl Mem st0 gv') /\
-smem_denotes_mem TD lc gl Mem sstate0.(SMem) mem' /\
-(forall st0,
-  In st0 sstate0.(Effects) ->
-  exists gv', sterm_denotes_genericvalue TD lc gl Mem st0 gv'
-  ).
+Hint Constructors sterm_denotes_genericvalue sterms_denote_genericvalues smem_denotes_mem.
+
+Definition smap_denotes_gvmap TD lc gl Mem sstate' lc' gl' :=
+(forall id' st' gv',  
+  binds id' st' sstate'.(STerms) ->
+  sterm_denotes_genericvalue TD lc gl Mem st' gv' ->
+  lookupEnv id' lc' gl' = Some gv') /\
+(forall id' gv',  
+  lookupEnv id' lc' gl' = Some gv' ->
+  exists st',
+   binds id' st' sstate'.(STerms) /\
+   sterm_denotes_genericvalue TD lc gl Mem st' gv'
+).
+
+Definition sstate_denotes_state TD lc gl Mem sstate' lc' gl' mem' :=
+smap_denotes_gvmap TD lc gl Mem sstate' lc' gl' /\
+smem_denotes_mem TD lc gl Mem sstate'.(SMem) mem'.
+
+Lemma subst_mt_in : forall sm id0 st0,
+  uniq sm ->
+  binds id0 st0 sm ->
+  subst_mt sm (sterm_val (value_id id0)) = st0.
+Admitted.
+
+Lemma subst_mt_notin : forall sm id0,
+  uniq sm ->
+  id0 `notin` dom sm ->
+  subst_mt sm (sterm_val (value_id id0)) = sterm_val (value_id id0).
+Admitted.
+
+Lemma subst_mt_const : forall sm c,
+  subst_mt sm (sterm_val (value_const c)) = sterm_val (value_const c).
+Admitted.
+
+       
+Lemma updateSmap_inversion : forall sm id0 st0 id1 st1,
+  uniq sm ->
+  binds id1 st1 (updateSmap sm id0 st0) ->
+  (id0 <> id1 /\ binds id1 st1 sm) \/ (id0 = id1 /\ st0 = st1).
+Proof.
+  induction sm; intros id0 st0 id1 st1 Uniq Binds; simpl in Binds.
+    analyze_binds Binds.
+
+    destruct a.
+    inversion Uniq; subst.
+    destruct (a==id0); subst.
+      analyze_binds Binds.
+      left. split; auto.
+        apply binds_In in BindsTac.
+        fsetdec.
+
+      analyze_binds Binds.
+      apply IHsm in BindsTac; auto.
+        destruct BindsTac; auto.
+          destruct H; auto.
+Qed.
+
+            
+Lemma binds_updateSmap_eq : forall sm id0 st0,
+  binds id0 st0 (updateSmap sm id0 st0).
+Proof.
+  induction sm; intros id0 st0; simpl; auto.
+    destruct a.
+    destruct (a == id0); subst; auto.
+Qed.
+
+Lemma binds_updateSmap_neq : forall sm id0 st0 id1 st1,
+  binds id1 st1 sm ->
+  id0 <> id1 ->
+  binds id1 st1 (updateSmap sm id0 st0).
+Proof.
+  induction sm; intros id0 st0 id1 st1 Hbinds id0_neq_id1; simpl; auto.
+    destruct a.
+    simpl_env in Hbinds.
+    analyze_binds Hbinds.
+      destruct (a == id0); subst; auto.
+        contradict id0_neq_id1; auto.
+
+      destruct (a == id0); subst; auto.
+Qed.
+
+Lemma genericvalue__implies__subst_mt_val_denotes : forall TD lc0 gl0 Mem0 sstate1 lc gl v gv,
+  uniq (STerms sstate1) ->
+  smap_denotes_gvmap TD lc0 gl0 Mem0 sstate1 lc gl ->
+  getOperandValue TD v lc gl = Some gv ->
+  sterm_denotes_genericvalue TD lc0 gl0 Mem0 (subst_mt (STerms sstate1) (sterm_val v)) gv.
+Proof.
+  intros D lc0 gl0 Mem0 sstate1 lc gl v gv Huniq Hdenotes J.
+  unfold getOperandValue in J.
+  unfold smap_denotes_gvmap in Hdenotes.
+  destruct Hdenotes as [J1 J2].
+  destruct v.
+    apply J2 in J.
+    destruct J as [st0 [J3 J4]].
+    rewrite subst_mt_in with (st0:=st0); auto.
+
+    rewrite subst_mt_const; auto.
+Qed.
+
+Lemma subst_mt_val_denotes__implies__genericvalue : forall TD lc0 gl0 Mem0 sstate1 lc gl v gv,
+  uniq (STerms sstate1) ->
+  (dom lc0 `union` dom gl0) [<=] dom (STerms sstate1) ->
+  smap_denotes_gvmap TD lc0 gl0 Mem0 sstate1 lc gl ->
+  sterm_denotes_genericvalue TD lc0 gl0 Mem0 (subst_mt (STerms sstate1) (sterm_val v)) gv ->
+  getOperandValue TD v lc gl = Some gv.
+Proof.
+  intros D lc0 gl0 Mem0 sstate1 lc gl v gv Huniq Hsub Hdenotes J.
+  unfold smap_denotes_gvmap in Hdenotes.
+  destruct Hdenotes as [J1 J2].
+  destruct v.
+    destruct (@AtomSetProperties.In_dec i0 (dom sstate1.(STerms))) as [i0_in_sstate1 | i0_notin_sstate1].
+      apply binds_In_inv in i0_in_sstate1.
+      destruct i0_in_sstate1 as [st0 Binds].
+      rewrite subst_mt_in with (st0:=st0) in J; auto.
+      apply J1 with (id':=i0) in J; auto.
+
+      rewrite subst_mt_notin in J; auto.
+      inversion J; subst.
+      simpl in H4.
+      apply lookupEnv__indom in H4.
+      clear - i0_notin_sstate1 H4 Hsub.
+      contradict H4; fsetdec.
+    rewrite subst_mt_const in J.
+    inversion J. auto.
+Qed.
+
+Lemma se_cmd__denotes__op_cmd__case1 : forall lc gl i0 gv3 lc' gl' id' st' sstate1 TD lc0 gl0 Mem0 gv',
+  updateEnv lc gl i0 gv3 = (lc', gl') ->
+  i0 <> id' ->
+  binds id' st' (STerms sstate1) ->
+  smap_denotes_gvmap TD lc0 gl0 Mem0 sstate1 lc gl ->
+  sterm_denotes_genericvalue TD lc0 gl0 Mem0 st' gv' ->
+  lookupEnv id' lc' gl' = Some gv'.
+Proof.
+  intros lc gl i0 gv3 lc' gl' id' st' sstate1 TD lc0 gl0 Mem0 gv' H25 nEQ Hbinds Hsterm_denotes Hdenotes.
+  apply lookupEnv_updateEnv_neq with (id1:=id') in H25; auto.
+  rewrite <- H25. 
+  unfold smap_denotes_gvmap in Hsterm_denotes.
+  destruct Hsterm_denotes as [J1 J2].
+  apply J1 with (st':=st'); auto.
+Qed.
+
+Lemma se_cmd__denotes__op_cmd__case2 : forall lc gl i0 gv3 lc' gl' id' sstate1 TD lc0 gl0 Mem0 gv' st0,
+  updateEnv lc gl i0 gv3 = (lc', gl') ->
+  smap_denotes_gvmap TD lc0 gl0 Mem0 sstate1 lc gl ->
+  lookupEnv id' lc' gl' = Some gv' ->
+  id' <> i0 ->
+  exists st', binds id' st' (updateSmap (STerms sstate1) i0 st0) /\ 
+              sterm_denotes_genericvalue TD lc0 gl0 Mem0 st' gv'.
+Proof.
+  intros lc gl i0 gv3 lc' gl' id' sstate1 TD lc0 gl0 Mem0 gv' st0 H25 Hsterm_denotes HlookupEnv n.
+  apply lookupEnv_updateEnv_neq with (id1:=id') in H25; auto.
+  rewrite <- H25 in HlookupEnv.
+  destruct Hsterm_denotes as [J1 J2].
+  apply J2 in HlookupEnv; auto.
+  destruct HlookupEnv as [st' [J3 J4]].
+  exists st'. split; auto.
+    apply binds_updateSmap_neq; auto.
+Qed.
+
+Lemma subst_mm_init : forall m0,
+  subst_mm m0 smem_init = smem_init.
+Proof.
+  induction m0; simpl; auto.
+    destruct a. auto.
+Qed.
+
+Lemma subst_mm_malloc : forall m0 sm1 t1 sz1 a1,
+  subst_mm m0 (smem_malloc sm1 t1 sz1 a1) = smem_malloc (subst_mm m0 sm1) t1 sz1 a1.
+Proof.
+  induction m0; simpl; intros; auto.
+    destruct a. auto.
+Qed.
+
+Lemma subst_mm_free : forall m0 sm1 t1 st1,
+  subst_mm m0 (smem_free sm1 t1 st1) = smem_free (subst_mm m0 sm1) t1 (subst_mt m0 st1).
+Proof.
+  induction m0; simpl; intros; auto.
+    destruct a. auto.
+Qed.
+
+Lemma subst_mm_alloca : forall m0 sm1 t1 sz1 a1,
+  subst_mm m0 (smem_alloca sm1 t1 sz1 a1) = smem_alloca (subst_mm m0 sm1) t1 sz1 a1.
+Proof.
+  induction m0; simpl; intros; auto.
+    destruct a. auto.
+Qed.
+
+Lemma subst_mm_smem_denotes_mem : forall TD lc gl Mem0 smem0 Mem1 smap0,
+  smem_denotes_mem TD lc gl Mem0 smem0 Mem1 <->
+  smem_denotes_mem TD lc gl Mem0 (subst_mm smap0 smem0) Mem1.
+Proof.
+  intros TD lc gl Mem0 smem0 Mem1 smap0.
+Admitted.
+
+Lemma smem_denotes_mem__implies__subst_mm : forall TD lc gl Mem0 smem0 Mem1 smap0,
+  smem_denotes_mem TD lc gl Mem0 smem0 Mem1 ->
+  smem_denotes_mem TD lc gl Mem0 (subst_mm smap0 smem0) Mem1.
+Admitted.
+
+Lemma subst_mm__implies__smem_denotes_mem : forall TD lc gl Mem0 smem0 Mem1 smap0,
+  smem_denotes_mem TD lc gl Mem0 (subst_mm smap0 smem0) Mem1 ->
+  smem_denotes_mem TD lc gl Mem0 smem0 Mem1.
+Admitted.
+
+Lemma smem_denotes_mem_det : forall TD lc gl Mem0 smem0 Mem1 Mem2,
+  smem_denotes_mem TD lc gl Mem0 smem0 Mem1 ->
+  smem_denotes_mem TD lc gl Mem0 smem0 Mem2 ->
+  Mem1 = Mem2.
+Admitted.
+
+Lemma se_cmd__denotes__op_cmd : forall S TD Ps F B c cs call0 sbs tmn lc arg als ECs gl lc0 gl0 Mem0 lc' als' gl' Mem1 Mem2 sstate1 tr,
+  dbCmd (mkState S TD Ps ((mkEC F B ((subblock_intro (c::cs) call0)::sbs) tmn lc arg als)::ECs) gl Mem1)
+         (mkState S TD Ps ((mkEC F B ((subblock_intro cs call0)::sbs) tmn lc' arg als')::ECs) gl' Mem2)
+         tr -> 
+  uniq sstate1.(STerms) ->
+  (dom lc0 `union` dom gl0) [<=] dom (STerms sstate1) ->
+  sstate_denotes_state TD lc0 gl0 Mem0 sstate1 lc gl Mem1 ->
+  sstate_denotes_state TD lc0 gl0 Mem0 (se_cmd sstate1 c) lc' gl' Mem2.
+Proof.
+  intros S TD Ps F B c cs call0 sbs tmn lc arg0 als ECs gl lc0 gl0 Mem0 lc' als' gl' Mem1 Mem2 sstate1 tr HdsInsn Huniq Hsub Hdenotes.
+  (cmd_cases (destruct c;
+              inversion HdsInsn; subst;
+              destruct Hdenotes as [Hsterm_denotes Hsmem_denotes]) Case).
+  Case "insn_bop".
+    split; auto.
+      split.
+        intros id' st' gv' Hbinds Hdenotes.
+        simpl in Hbinds. simpl_env in Hbinds.
+        analyze_binds Hbinds.
+        apply updateSmap_inversion in Hbinds; auto.
+        destruct Hbinds as [[nEQ Hbinds] | [EQ1 EQ2]]; subst.
+          eapply se_cmd__denotes__op_cmd__case1; eauto.
+
+          apply lookupEnv_updateEnv_eq in H25; auto.
+          rewrite H25.
+          inversion Hdenotes; subst.
+          unfold BOP in H24.
+          apply subst_mt_val_denotes__implies__genericvalue with (lc:=lc)(gl:=gl) in H8; auto.
+          apply subst_mt_val_denotes__implies__genericvalue with (lc:=lc)(gl:=gl) in H9; auto.
+          rewrite H8 in H24. rewrite H9 in H24.
+          rewrite H24 in H10. auto.
+
+        intros id' gv' HlookupEnv.
+        simpl. 
+        destruct (id'==i0); subst.
+          exists (sterm_bop b s (subst_mt (STerms sstate1) (sterm_val v)) (subst_mt (STerms sstate1) (sterm_val v0))).
+          split. 
+            apply binds_updateSmap_eq; auto.
+
+            apply lookupEnv_updateEnv_eq in H25; auto.
+            rewrite H25 in HlookupEnv.
+            inversion HlookupEnv; subst.
+            apply BOP_inversion in H24.
+            destruct H24 as [gv1 [gv2 [J1 [J2 J3]]]].
+            apply sterm_bop_denotes with (gv1:=gv1)(gv2:=gv2); eauto using genericvalue__implies__subst_mt_val_denotes.
+
+          eapply se_cmd__denotes__op_cmd__case2; eauto.
+
+  Case "insn_extractvalue".
+    split; auto.
+      split.
+        intros id' st' gv'0 Hbinds Hdenotes.
+        simpl in Hbinds. simpl_env in Hbinds.
+        analyze_binds Hbinds.
+        apply updateSmap_inversion in Hbinds; auto.
+        destruct Hbinds as [[nEQ Hbinds] | [EQ1 EQ2]]; subst.
+          eapply se_cmd__denotes__op_cmd__case1; eauto.
+
+          apply lookupEnv_updateEnv_eq in H25; auto.
+          rewrite H25.
+          inversion Hdenotes; subst.
+          apply subst_mt_val_denotes__implies__genericvalue with (lc:=lc)(gl:=gl) in H7; auto.
+          rewrite H7 in H23. inversion H23; subst.
+          rewrite H24 in H8. auto.
+
+        intros id' gv'0 HlookupEnv.
+        simpl. 
+        destruct (id'==i0); subst.
+          exists (sterm_extractvalue t (subst_mt (STerms sstate1) (sterm_val v)) l0).
+          split. 
+            apply binds_updateSmap_eq; auto.
+
+            apply lookupEnv_updateEnv_eq in H25; auto.
+            rewrite H25 in HlookupEnv.
+            inversion HlookupEnv; subst.
+            apply sterm_extractvalue_denotes with (gv1:=gv); eauto using genericvalue__implies__subst_mt_val_denotes.
+
+          eapply se_cmd__denotes__op_cmd__case2; eauto.
+
+  Case "insn_insertvalue".
+    split; auto.
+      split.
+        intros id' st' gv'0 Hbinds Hdenotes.
+        simpl in Hbinds. simpl_env in Hbinds.
+        analyze_binds Hbinds.
+        apply updateSmap_inversion in Hbinds; auto.
+        destruct Hbinds as [[nEQ Hbinds] | [EQ1 EQ2]]; subst.
+          eapply se_cmd__denotes__op_cmd__case1; eauto.
+
+          apply lookupEnv_updateEnv_eq in H28; auto.
+          rewrite H28.
+          inversion Hdenotes; subst.
+          apply subst_mt_val_denotes__implies__genericvalue with (lc:=lc)(gl:=gl) in H9; auto.
+          apply subst_mt_val_denotes__implies__genericvalue with (lc:=lc)(gl:=gl) in H10; auto.
+          rewrite H9 in H25. inversion H25; subst.
+          rewrite H10 in H26. inversion H26; subst.
+          rewrite H27 in H11. auto.
+
+        intros id' gv'0 HlookupEnv.
+        simpl. 
+        destruct (id'==i0); subst.
+          exists (sterm_insertvalue t (subst_mt (STerms sstate1) (sterm_val v)) t0 (subst_mt (STerms sstate1) (sterm_val v0)) l0).
+          split. 
+            apply binds_updateSmap_eq; auto.
+
+            apply lookupEnv_updateEnv_eq in H28; auto.
+            rewrite H28 in HlookupEnv.
+            inversion HlookupEnv; subst.
+            eapply sterm_insertvalue_denotes; eauto using genericvalue__implies__subst_mt_val_denotes.
+
+          eapply se_cmd__denotes__op_cmd__case2; eauto.
+
+  Case "insn_malloc".
+    split.
+      split.
+        intros id' st' gv'0 Hbinds Hdenotes.
+        simpl in Hbinds. simpl_env in Hbinds.
+        analyze_binds Hbinds.
+        apply updateSmap_inversion in Hbinds; auto.
+        destruct Hbinds as [[nEQ Hbinds] | [EQ1 EQ2]]; subst.
+          eapply se_cmd__denotes__op_cmd__case1; eauto.
+
+          apply lookupEnv_updateEnv_eq in H25; auto.
+          rewrite H25.
+          inversion Hdenotes; subst. 
+          apply subst_mm__implies__smem_denotes_mem in H8; auto.
+          apply smem_denotes_mem_det with (Mem2:=Mem1) in H8; auto.
+          subst.
+          rewrite H9 in H23. inversion H23; subst.
+          rewrite H10 in H24. inversion H24; auto.
+     
+        intros id' gv'0 HlookupEnv.
+        simpl.
+        destruct (id'==i0); subst.
+          exists (sterm_malloc (subst_mm (STerms sstate1) (SMem sstate1)) t s a).
+          split. 
+            apply binds_updateSmap_eq; auto.
+
+            apply lookupEnv_updateEnv_eq in H25; auto.
+            rewrite H25 in HlookupEnv.
+            inversion HlookupEnv; subst.
+            eapply sterm_malloc_denotes; eauto using smem_denotes_mem__implies__subst_mm.
+
+          eapply se_cmd__denotes__op_cmd__case2; eauto.
+
+      simpl. eauto using smem_denotes_mem__implies__subst_mm.
+
+  Case "insn_free".
+    split; simpl.
+      destruct Hsterm_denotes as [J1 J2].
+      split; auto.
+     
+      apply getOperandPtr_inversion in H22.
+      destruct H22 as [gv [J1 J2]].
+      apply smem_free_denotes with (Mem1:=Mem1)(gv0:=gv)(mptr0:=mptr); auto.
+        eapply genericvalue__implies__subst_mt_val_denotes; eauto.
+    
+  Case "insn_alloca".
+    split.
+      split.
+        intros id' st' gv'0 Hbinds Hdenotes.
+        simpl in Hbinds. simpl_env in Hbinds.
+        analyze_binds Hbinds.
+        apply updateSmap_inversion in Hbinds; auto.
+        destruct Hbinds as [[nEQ Hbinds] | [EQ1 EQ2]]; subst.
+          eapply se_cmd__denotes__op_cmd__case1; eauto.
+
+          apply lookupEnv_updateEnv_eq in H25; auto.
+          rewrite H25.
+          inversion Hdenotes; subst. 
+          apply subst_mm__implies__smem_denotes_mem in H8; auto.
+          apply smem_denotes_mem_det with (Mem2:=Mem1) in H8; auto.
+          subst.
+          rewrite H9 in H23. inversion H23; subst.
+          rewrite H10 in H24. inversion H24; auto.
+     
+        intros id' gv'0 HlookupEnv.
+        simpl.
+        destruct (id'==i0); subst.
+          exists (sterm_alloca (subst_mm (STerms sstate1) (SMem sstate1)) t s a).
+          split. 
+            apply binds_updateSmap_eq; auto.
+
+            apply lookupEnv_updateEnv_eq in H25; auto.
+            rewrite H25 in HlookupEnv.
+            inversion HlookupEnv; subst.
+            eapply sterm_alloca_denotes; eauto using smem_denotes_mem__implies__subst_mm.
+
+          eapply se_cmd__denotes__op_cmd__case2; eauto.
+
+      simpl. eauto using smem_denotes_mem__implies__subst_mm.
+
+  Case "insn_load".
+    split.
+      apply getOperandPtr_inversion in H22.
+      destruct H22 as [gv2 [J1 J2]].
+      split.
+        intros id' st' gv'0 Hbinds Hdenotes.
+        simpl in Hbinds. simpl_env in Hbinds.
+        analyze_binds Hbinds.
+        apply updateSmap_inversion in Hbinds; auto.
+        destruct Hbinds as [[nEQ Hbinds] | [EQ1 EQ2]]; subst.
+          eapply se_cmd__denotes__op_cmd__case1; eauto.
+
+          apply lookupEnv_updateEnv_eq in H24; auto.
+          rewrite H24.
+          inversion Hdenotes; subst. 
+          apply subst_mm__implies__smem_denotes_mem in H7; auto.
+          apply smem_denotes_mem_det with (Mem2:=Mem2) in H7; auto.
+          subst.
+          apply subst_mt_val_denotes__implies__genericvalue with (lc:=lc)(gl:=gl) in H2; auto.
+          rewrite J1 in H2. inversion H2; subst.
+          rewrite H9 in J2. inversion J2; subst.
+          rewrite H23 in H10. auto.
+     
+        intros id' gv'0 HlookupEnv.
+        simpl.
+        destruct (id'==i0); subst.
+          exists (sterm_load (subst_mm (STerms sstate1) (SMem sstate1)) t (subst_mt (STerms sstate1) (sterm_val v))).
+          split. 
+            apply binds_updateSmap_eq; auto.
+
+            apply lookupEnv_updateEnv_eq in H24; auto.
+            rewrite H24 in HlookupEnv.
+            inversion HlookupEnv; subst.
+            apply sterm_load_denotes with (Mem1:=Mem2)(gv0:=gv2)(mp0:=mp); eauto using smem_denotes_mem__implies__subst_mm.
+              eapply genericvalue__implies__subst_mt_val_denotes; eauto.
+
+          eapply se_cmd__denotes__op_cmd__case2; eauto.
+
+      simpl. eauto using smem_denotes_mem__implies__subst_mm.
+
+  Case "insn_store".
+    split; simpl.
+      destruct Hsterm_denotes as [J1 J2].
+      split; auto.
+
+      apply getOperandPtr_inversion in H24.
+      destruct H24 as [gv2 [J1 J2]].
+      eapply smem_store_denotes; 
+        eauto using smem_denotes_mem__implies__subst_mm, 
+                    genericvalue__implies__subst_mt_val_denotes.
+
+  Case "insn_gep". 
+    split; auto.
+      split.
+        intros id' st' gv' Hbinds Hdenotes.
+        simpl in Hbinds. simpl_env in Hbinds.
+        analyze_binds Hbinds.
+        apply updateSmap_inversion in Hbinds; auto.
+        apply getOperandPtr_inversion in H24.
+        destruct H24 as [gv0 [J1 J2]].
+        destruct Hbinds as [[nEQ Hbinds] | [EQ1 EQ2]]; subst.
+          eapply se_cmd__denotes__op_cmd__case1; eauto.
+
+          apply lookupEnv_updateEnv_eq in H26; auto.
+          rewrite H26.
+          inversion Hdenotes; subst.
+          unfold GEP in H25.
+          apply subst_mt_val_denotes__implies__genericvalue with (lc:=lc)(gl:=gl) in H3; auto.
+          rewrite H3 in J1. inversion J1; subst.
+          admit.
+
+        intros id' gv' HlookupEnv.
+        simpl. 
+        destruct (id'==i0); subst.
+          exists (sterm_gep i1 t (subst_mt (STerms sstate1) (sterm_val v)) (List.map (subst_mt (STerms sstate1)) (List.map sterm_val l0))).
+          split. 
+            apply binds_updateSmap_eq; auto.
+
+            apply lookupEnv_updateEnv_eq in H26; auto.
+            rewrite H26 in HlookupEnv.
+            inversion HlookupEnv; subst.
+            apply getOperandPtr_inversion in H24.
+            destruct H24 as [gv0 [J1 J2]].
+(*
+            eapply sterm_gep_denotes; eauto using genericvalue__implies__subst_mt_val_denotes.
+*)
+            admit.
+
+          eapply se_cmd__denotes__op_cmd__case2; eauto.
+
+  Case "insn_ext".
+    split; auto.
+      split.
+        intros id' st' gv' Hbinds Hdenotes.
+        simpl in Hbinds. simpl_env in Hbinds.
+        analyze_binds Hbinds.
+        apply updateSmap_inversion in Hbinds; auto.
+        destruct Hbinds as [[nEQ Hbinds] | [EQ1 EQ2]]; subst.
+          eapply se_cmd__denotes__op_cmd__case1; eauto.
+
+          apply lookupEnv_updateEnv_eq in H25; auto.
+          rewrite H25.
+          inversion Hdenotes; subst.
+          unfold EXT in H24.
+          apply subst_mt_val_denotes__implies__genericvalue with (lc:=lc)(gl:=gl) in H8; auto.
+          rewrite H8 in H24.
+          rewrite H24 in H9. auto.
+
+        intros id' gv' HlookupEnv.
+        simpl. 
+        destruct (id'==i0); subst.
+          exists (sterm_ext e t (subst_mt (STerms sstate1) (sterm_val v)) t0).
+          split. 
+            apply binds_updateSmap_eq; auto.
+
+            apply lookupEnv_updateEnv_eq in H25; auto.
+            rewrite H25 in HlookupEnv.
+            inversion HlookupEnv; subst.
+            apply EXT_inversion in H24.
+            destruct H24 as [gv1 [J1 J2]].
+            apply sterm_ext_denotes with (gv1:=gv1); eauto using genericvalue__implies__subst_mt_val_denotes.
+
+          eapply se_cmd__denotes__op_cmd__case2; eauto.
+
+  Case "insn_cast".
+    split; auto.
+      split.
+        intros id' st' gv' Hbinds Hdenotes.
+        simpl in Hbinds. simpl_env in Hbinds.
+        analyze_binds Hbinds.
+        apply updateSmap_inversion in Hbinds; auto.
+        destruct Hbinds as [[nEQ Hbinds] | [EQ1 EQ2]]; subst.
+          eapply se_cmd__denotes__op_cmd__case1; eauto.
+
+          apply lookupEnv_updateEnv_eq in H25; auto.
+          rewrite H25.
+          inversion Hdenotes; subst.
+          unfold CAST in H24.
+          apply subst_mt_val_denotes__implies__genericvalue with (lc:=lc)(gl:=gl) in H8; auto.
+          rewrite H8 in H24.
+          rewrite H24 in H9. auto.
+
+        intros id' gv' HlookupEnv.
+        simpl. 
+        destruct (id'==i0); subst.
+          exists (sterm_cast c t (subst_mt (STerms sstate1) (sterm_val v)) t0).
+          split. 
+            apply binds_updateSmap_eq; auto.
+
+            apply lookupEnv_updateEnv_eq in H25; auto.
+            rewrite H25 in HlookupEnv.
+            inversion HlookupEnv; subst.
+            apply CAST_inversion in H24.
+            destruct H24 as [gv1 [J1 J2]].
+            apply sterm_cast_denotes with (gv1:=gv1); eauto using genericvalue__implies__subst_mt_val_denotes.
+
+          eapply se_cmd__denotes__op_cmd__case2; eauto.
+
+  Case "insn_icmp".
+    split; auto.
+      split.
+        intros id' st' gv' Hbinds Hdenotes.
+        simpl in Hbinds. simpl_env in Hbinds.
+        analyze_binds Hbinds.
+        apply updateSmap_inversion in Hbinds; auto.
+        destruct Hbinds as [[nEQ Hbinds] | [EQ1 EQ2]]; subst.
+          eapply se_cmd__denotes__op_cmd__case1; eauto.
+
+          apply lookupEnv_updateEnv_eq in H25; auto.
+          rewrite H25.
+          inversion Hdenotes; subst.
+          unfold ICMP in H24.
+          apply subst_mt_val_denotes__implies__genericvalue with (lc:=lc)(gl:=gl) in H8; auto.
+          apply subst_mt_val_denotes__implies__genericvalue with (lc:=lc)(gl:=gl) in H9; auto.
+          rewrite H8 in H24. rewrite H9 in H24.
+          rewrite H24 in H10. auto.
+
+        intros id' gv' HlookupEnv.
+        simpl. 
+        destruct (id'==i0); subst.
+          exists (sterm_icmp c t (subst_mt (STerms sstate1) (sterm_val v)) (subst_mt (STerms sstate1) (sterm_val v0))).
+          split. 
+            apply binds_updateSmap_eq; auto.
+
+            apply lookupEnv_updateEnv_eq in H25; auto.
+            rewrite H25 in HlookupEnv.
+            inversion HlookupEnv; subst.
+            apply ICMP_inversion in H24.
+            destruct H24 as [gv1 [gv2 [J1 [J2 J3]]]].
+            apply sterm_icmp_denotes with (gv1:=gv1)(gv2:=gv2); eauto using genericvalue__implies__subst_mt_val_denotes.
+
+          eapply se_cmd__denotes__op_cmd__case2; eauto.
+
+  Case "insn_select".
+    split; auto.
+      split.
+        intros id' st' gv' Hbinds Hdenotes.
+        simpl in Hbinds. simpl_env in Hbinds.
+        analyze_binds Hbinds.
+        apply updateSmap_inversion in Hbinds; auto.
+        destruct Hbinds as [[nEQ Hbinds] | [EQ1 EQ2]]; subst.
+          destruct cond0; eapply se_cmd__denotes__op_cmd__case1; eauto.
+
+          symmetry in H27.
+          inversion Hdenotes; subst.
+          apply subst_mt_val_denotes__implies__genericvalue with (lc:=lc)(gl:=gl) in H3; auto.
+          apply subst_mt_val_denotes__implies__genericvalue with (lc:=lc)(gl:=gl) in H8; auto.
+          apply subst_mt_val_denotes__implies__genericvalue with (lc:=lc)(gl:=gl) in H10; auto.
+          apply getOperandInt_inversion in H24. destruct H24 as [gv5 [J1 J2]].
+          rewrite H3 in J1. inversion J1; subst.
+          rewrite H8 in H25. inversion H25; subst.
+          rewrite H10 in H26. inversion H26; subst.
+          rewrite H11 in J2. inversion J2; subst.
+          destruct cond0; apply lookupEnv_updateEnv_eq in H27; auto.
+
+        intros id' gv' HlookupEnv.
+        simpl. 
+        destruct (id'==i0); subst.
+          exists (sterm_select (subst_mt (STerms sstate1) (sterm_val v)) t (subst_mt (STerms sstate1) (sterm_val v0))  (subst_mt (STerms sstate1) (sterm_val v1))).
+          split. 
+            apply binds_updateSmap_eq; auto.
+
+            apply getOperandInt_inversion in H24. destruct H24 as [gv5 [J1 J2]].
+            apply sterm_select_denotes with (c0:=cond0)(gv0:=gv5)(gv1:=gv1)(gv2:=gv2); eauto using genericvalue__implies__subst_mt_val_denotes.
+            symmetry in H27.
+            destruct cond0;
+              apply lookupEnv_updateEnv_eq in H27; auto;
+              rewrite H27 in HlookupEnv;
+              inversion HlookupEnv; subst; auto.
+
+          destruct cond0; eapply se_cmd__denotes__op_cmd__case2; eauto.
+Qed.
+
+Lemma dbCmd_inversion : forall a cs S TD Ps F B call0 sbs tmn arg als ECs lc gl Mem1 state2 tr,
+  dbCmd (mkState S TD Ps ((mkEC F B ((subblock_intro (a::cs) call0)::sbs) tmn lc arg als)::ECs) gl Mem1)
+        state2
+        tr ->
+  exists lc', exists gl', exists als', exists Mem2,
+    state2 = (mkState S TD Ps ((mkEC F B ((subblock_intro cs call0)::sbs) tmn lc' arg als')::ECs) gl' Mem2).
+Proof.
+  intros a cs S TD Ps F B call0 sbs tmn arg0 als ECs lc gl Mem1 state2 tr HdbCmd.
+  inversion HdbCmd; subst; 
+  try solve [
+    exists lc'; exists gl'; exists als; exists Mem1; auto |
+    exists lc'; exists gl'; exists als; exists Mem'; auto |
+    exists lc; exists gl; exists als; exists Mem'; auto |
+    exists lc'; exists gl'; exists (mb::als); exists Mem'; auto
+  ].
+Qed.
+
+Lemma updateSmap_dom_eq : forall sm id0 st0,
+  dom (updateSmap sm id0 st0) [=] dom sm `union` {{id0}}.
+Proof.
+  induction sm; intros; simpl; try solve [fsetdec].
+    destruct a. 
+    destruct (a==id0); simpl; try solve [fsetdec].
+      assert (J:=@IHsm id0 st0). fsetdec.
+Qed.
+
+Lemma updateSmap_uniq : forall sm id0 st0,
+  uniq sm ->
+  uniq (updateSmap sm id0 st0).
+Proof.
+  induction sm; intros; simpl; auto.
+    destruct a.
+
+    destruct_uniq.
+    destruct (a==id0); subst; try solve [solve_uniq].
+      apply IHsm with (id0:=id0)(st0:=st0) in H. 
+      assert (J:=@updateSmap_dom_eq sm id0 st0).
+      solve_uniq.
+Qed.
+
+Lemma se_cmd_uniq : forall sstate0 c,
+  uniq (STerms sstate0) ->
+  uniq (STerms (se_cmd sstate0 c)).
+Proof.
+  intros sstate0 c Huniq.
+  destruct c; simpl; try solve [apply updateSmap_uniq; auto | auto].
+Qed.
+
+Lemma se_cmd_dom_mono : forall sstate0 c,
+  dom (STerms sstate0) [<=] dom (STerms (se_cmd sstate0 c)).
+Proof.
+  intros sstate0 c.
+  assert (forall sm id0 st0, dom sm [<=] dom (updateSmap sm id0 st0)) as J.
+    intros. assert (J:=@updateSmap_dom_eq sm id0 st0). fsetdec. 
+  destruct c; simpl; try solve [eauto using J| fsetdec].
+Qed.
+
+Lemma aux__se_cmds__denotes__op_cmds : forall cs S TD Ps F B call0 sbs tmn lc0 arg als ECs gl0 Mem0 lc als' gl Mem1 sstate1 lc' gl' Mem2 tr,
+  dbCmds (mkState S TD Ps ((mkEC F B ((subblock_intro cs call0)::sbs) tmn lc arg als)::ECs) gl Mem1)
+         (mkState S TD Ps ((mkEC F B ((subblock_intro nil call0)::sbs) tmn lc' arg als')::ECs) gl' Mem2)
+         tr ->
+  uniq sstate1.(STerms) ->
+  (dom lc0 `union` dom gl0) [<=] dom (STerms sstate1) ->
+  sstate_denotes_state TD lc0 gl0 Mem0 sstate1 lc gl Mem1 ->
+  sstate_denotes_state TD lc0 gl0 Mem0 (se_cmds sstate1 cs) lc' gl' Mem2.
+Proof.
+  induction cs; 
+    intros S TD Ps F B call0 sbs tmn lc0 arg0 als ECs gl0 Mem0 lc als' gl Mem1 sstate1 lc' gl' Mem2 tr HdbCmds Huniq Hsub Hdenotes.
+
+    inversion HdbCmds; subst; auto.
+      inversion H.
+
+    inversion HdbCmds; subst.
+    assert (Hcmd:=H).
+    apply dbCmd_inversion in H.
+    destruct H as [lc3 [gl3 [als3 [Mem3 H]]]]; subst.
+    simpl.
+    apply se_cmd__denotes__op_cmd with (lc0:=lc0)(gl0:=gl0)(sstate1:=sstate1)(Mem0:=Mem0) in Hcmd; auto.
+    apply IHcs with (lc0:=lc0)(gl0:=gl0)(sstate1:=se_cmd sstate1 a)(Mem0:=Mem0) in H0; auto.
+      apply se_cmd_uniq; auto.
+
+      assert (J:=@se_cmd_dom_mono sstate1 a).
+      clear - J Hsub. fsetdec.
+Qed.
+
+Fixpoint globals_to_smap (gl:GVMap) : smap :=
+match gl with
+| nil => nil
+| (id0, _)::gl' => updateSmap (globals_to_smap gl') id0 (sterm_val (value_id id0)) 
+end.
+
+Fixpoint locals_to_smap (lc:GVMap) (m0:smap) : smap :=
+match lc with
+| nil => m0
+| (id0, _)::lc' => updateSmap (locals_to_smap lc' m0) id0 (sterm_val (value_id id0)) 
+end.
+
+Definition env_to_smap (gl lc:GVMap) : smap :=
+locals_to_smap lc (globals_to_smap gl).
+
+Lemma globals_to_smap_dom_eq : forall gl,
+  dom (globals_to_smap gl) [=] dom gl.
+Proof.
+  induction gl; simpl.
+    fsetdec.
+
+    destruct a.
+    rewrite <- IHgl. clear IHgl.
+    rewrite updateSmap_dom_eq. fsetdec.
+Qed.
+
+Lemma locals_to_smap_dom_eq : forall lc m0,
+  dom (locals_to_smap lc m0) [=] dom lc `union` dom m0.
+Proof.
+  induction lc; intros m0; simpl.
+    fsetdec.
+
+    destruct a.
+    rewrite updateSmap_dom_eq. 
+    rewrite IHlc.
+    fsetdec.
+Qed.
+
+Lemma env_to_smap_dom_eq : forall gl lc,
+  dom (env_to_smap gl lc) [=] dom gl `union` dom lc.
+Proof.
+  intros gl lc.
+  unfold env_to_smap.
+  rewrite locals_to_smap_dom_eq.
+  rewrite globals_to_smap_dom_eq.
+  fsetdec.
+Qed.
+
+Lemma globals_to_smap_uniq : forall gl,
+  uniq (globals_to_smap gl).
+Proof.
+  induction gl; simpl; auto.
+    destruct a.
+    apply updateSmap_uniq; auto.
+Qed.
+
+Lemma locals_to_smap_uniq : forall lc m0,
+  uniq m0 ->
+  uniq (locals_to_smap lc m0).
+Proof.
+  induction lc; simpl; intros; auto.
+    destruct a.
+    apply updateSmap_uniq; auto.
+Qed.
+
+Lemma env_to_smap_uniq : forall gl lc,
+  uniq (env_to_smap gl lc).
+Proof.
+  intros gl lc.
+  unfold env_to_smap.
+  apply locals_to_smap_uniq.
+  apply globals_to_smap_uniq.
+Qed.
+
+Lemma binds_env_to_smap : forall id0 st0 gl lc,
+  binds id0 st0 (env_to_smap gl lc) ->
+  st0 = sterm_val (value_id id0).
+Proof.
+Admitted.
+
+Lemma env_to_smap_denotes__imples__gv : forall id0 st0 TD Mem0 gl lc gv0,
+  binds id0 st0 (env_to_smap gl lc) ->
+  sterm_denotes_genericvalue TD lc gl Mem0 st0 gv0 ->
+  lookupEnv id0 lc gl = Some gv0.
+Proof.
+  intros id0 st0 TD Mem0 gl lc gv0 Binds Denotes.
+  apply binds_env_to_smap in Binds.
+  rewrite Binds in Denotes.
+  inversion Denotes; subst.
+  simpl in H4. auto.
+Qed.
+
+Lemma lookupEnv_env_to_smap : forall id0 gv0 gl lc,
+  lookupEnv id0 lc gl = Some gv0 ->
+  binds id0 (sterm_val (value_id id0)) (env_to_smap gl lc).
+Proof.
+Admitted.
+
+Lemma gv__imples__env_to_smap_denotes : forall id0 TD Mem0 gl lc gv0,
+  lookupEnv id0 lc gl = Some gv0 ->
+  binds id0 (sterm_val (value_id id0)) (env_to_smap gl lc) /\
+  sterm_denotes_genericvalue TD lc gl Mem0 (sterm_val (value_id id0)) gv0.
+Proof.
+  intros id0 TD Mem0 gl lc gv0 Binds.
+  split.
+    eapply lookupEnv_env_to_smap; eauto.
+
+    apply sterm_val_denotes; auto.
+Qed.
+
+Lemma se_cmds__denotes__op_cmds : forall S TD Ps F B cs call0 sbs tmn lc arg als ECs gl Mem lc' als' gl' Mem' tr,
+  dbCmds (mkState S TD Ps ((mkEC F B ((subblock_intro cs call0)::sbs) tmn lc arg als)::ECs) gl Mem)
+         (mkState S TD Ps ((mkEC F B ((subblock_intro nil call0)::sbs) tmn lc' arg als')::ECs) gl' Mem')
+         tr ->
+  sstate_denotes_state TD lc gl Mem (se_cmds (mkSstate (env_to_smap gl lc) smem_init) cs) lc' gl' Mem'.
+Proof.
+  intros S TD Ps F B cs call0 sbs tmn lc arg0 als ECs gl Mem0 lc' als' gl' Mem' tr HdbCmds.
+  apply aux__se_cmds__denotes__op_cmds with (lc0:=lc)(gl0:=gl)(Mem0:=Mem0)(sstate1:=mkSstate (env_to_smap gl lc) smem_init) in HdbCmds; simpl; auto.
+    apply env_to_smap_uniq.
+
+    rewrite env_to_smap_dom_eq. fsetdec.
+
+    split; simpl; auto.
+      unfold smap_denotes_gvmap.
+      split; intros.
+        simpl in H.
+        apply env_to_smap_denotes__imples__gv with (id0:=id') in H0; auto.
+
+        exists (sterm_val (value_id id')).
+        apply gv__imples__env_to_smap_denotes; auto.
+Qed.           
+
+Definition se_subblock (st : sstate) (b:subblock) : sstate*scall :=
+match b with
+| subblock_intro cs call0 =>
+  let st0 := se_cmds st cs in
+  (st0, se_call st0 call0)
+end.
+
+Definition tv_subblock (b1 b2:subblock) :=
+match (b1, b2) with
+| (subblock_intro cs1 call1, subblock_intro cs2 call2) =>
+  match (call1, call2) with
+  | (insn_call id1 _ _ _ _ _, insn_call id2 _ _ _ _ _) => 
+    if id1==id2 
+    then
+      let st1 := se_cmds (mkSstate nil smem_init) cs1 in
+      let st2 := se_cmds (mkSstate nil smem_init) cs2 in
+      let cl1 := se_call st1 call1 in
+      let cl2 := se_call st2 call2 in
+      st1 = st2 /\ cl1 = cl2
+    else
+      False
+  end
+end.
+
+End SimpleSE.
+
