src/ssa/genericvalues.v
@@ -1,0 +1,630 @@
+Add LoadPath "./ott".
+Add LoadPath "./monads".
+Add LoadPath "../../../theory/metatheory".
+Require Import ssa.
+Require Import List.
+Require Import Arith.
+Require Import ssa_mem.
+Require Import monad.
+Require Import trace.
+Require Import Metatheory.
+
+Definition GenericValue := mvalue.
+Definition GV2nat := mvalue2nat.
+Definition GV2ptr := mvalue2mptr.
+Definition isGVUndef := isMvalueUndef.
+Definition nat2GV := nat2mvalue.
+Definition undef2GV := undef2mvalue.
+Definition ptr2GV TD p := mptr2mvalue TD p (getPointerSizeInBits TD).
+
+Definition GVMap := list (id*GenericValue).
+
+(* update if exists, add it otherwise *)
+Fixpoint updateAddGVMap (m:GVMap) (i:id) (gv:GenericValue) : GVMap :=
+match m with
+| nil => (i, gv)::nil
+| (i', gv')::m' =>
+  if (eq_dec i i')
+  then (i', gv)::m'
+  else (i', gv')::updateAddGVMap m' i gv
+end.
+
+(* update only if exists, do nothing otherwise *)
+Fixpoint updateGVMap (m:GVMap) (i:id) (gv:GenericValue) : GVMap :=
+match m with
+| nil => nil
+| (i', gv')::m' =>
+  if (eq_dec i i')
+  then (i', gv)::m'
+  else (i', gv')::updateGVMap m' i gv
+end.
+
+Fixpoint lookupGVMap (m:GVMap) (i:id) : option GenericValue :=
+match m with
+| nil => None
+| (i', gv')::m' =>
+  if (eq_dec i i')
+  then Some gv'
+  else lookupGVMap m' i
+end.
+
+(* Globals are fixed at runtime, only changed when genGlobalAndInitMem;
+   but locals can be changed. 
+   Update Locals if id exists locally,
+   Add it into Locals if id isnt in locals and globals,
+   if the id is shadowed by locals, then update globals. *)
+Definition updateEnv (locals globals:GVMap) (i:id) (gv:GenericValue) : GVMap*GVMap :=
+if (@AtomSetProperties.In_dec i (dom locals))
+then (* i is in locals *) 
+  (updateGVMap locals i gv, globals)
+else (* i isnt in locals, *)
+  if (@AtomSetProperties.In_dec i (dom globals))
+  then (* but i is in globals *) 
+    (locals, updateGVMap globals i gv)
+  else (* i is fresh. *) 
+    (updateAddGVMap locals i gv, globals)
+.
+
+Definition lookupEnv (i:id) (locals:GVMap) (globals:GVMap) : option GenericValue := 
+match lookupGVMap locals i with
+| Some gv => Some gv
+| None => lookupGVMap globals i
+end.
+
+Lemma lookupGVMap_updateGVMap_in : forall m id0 gv0,
+  id0 `in` dom m ->
+  lookupGVMap (updateGVMap m id0 gv0) id0 = Some gv0.
+Proof.
+  induction m; intros; simpl.
+    simpl in H. contradict H; auto.
+
+    destruct a.
+    destruct (@eq_dec id (@EqDec_eq_of_EqDec id EqDec_atom) id0 a); subst; simpl.
+      destruct (@eq_dec id (@EqDec_eq_of_EqDec id EqDec_atom) a a); subst; simpl; auto.
+        contradict n; auto.
+      destruct (@eq_dec id (@EqDec_eq_of_EqDec id EqDec_atom) id0 a); subst; simpl; auto.
+        contradict n; auto.
+
+        assert (id0 = a \/ id0 `in` dom m) as J. simpl in H. fsetdec.
+        destruct J as [J | J]; subst.
+          contradict n; auto.
+          apply IHm with (gv0:=gv0) in J; auto.
+Qed.   
+
+Lemma lookupGVMap_updateAddGVMap_eq : forall m id0 gv0,
+  lookupGVMap (updateAddGVMap m id0 gv0) id0 = Some gv0.
+Proof.
+  induction m; intros; simpl.
+    destruct (@eq_dec id (@EqDec_eq_of_EqDec id EqDec_atom) id0 id0); subst; simpl; auto.
+      contradict n; auto.  
+
+    destruct a.
+    destruct (@eq_dec id (@EqDec_eq_of_EqDec id EqDec_atom) id0 i0); subst; simpl.
+      destruct (@eq_dec id (@EqDec_eq_of_EqDec id EqDec_atom) i0 i0); subst; simpl; auto.
+        contradict n; auto.
+      destruct (@eq_dec id (@EqDec_eq_of_EqDec id EqDec_atom) id0 i0); subst; simpl; auto.
+        contradict n; auto.
+Qed.   
+
+Lemma lookupGVMap_notin : forall m id0,
+  id0 `notin` dom m ->
+  lookupGVMap m id0 = None.
+Proof.
+  induction m; intros; simpl; auto.
+    destruct a.
+    simpl in H. 
+    destruct (@eq_dec id (@EqDec_eq_of_EqDec id EqDec_atom) id0 a); subst; simpl; auto.
+      contradict H; auto.
+Qed.
+
+Lemma lookupEnv_updateEnv_eq : forall id0 lc gl gv0 lc' gl',
+  updateEnv lc gl id0 gv0 = (lc', gl') ->
+  lookupEnv id0 lc' gl' = Some gv0.
+Proof.
+  intros id0 lc gl gv0 lc' gl' HupdateEnv.
+  unfold lookupEnv.
+  unfold updateEnv in HupdateEnv.
+  destruct (@AtomSetProperties.In_dec id0 (dom lc)) as [id0_in_lc | id0_notin_lc].
+    inversion HupdateEnv; subst. clear HupdateEnv.
+    rewrite lookupGVMap_updateGVMap_in; auto.
+
+    destruct (@AtomSetProperties.In_dec id0 (dom gl)) as [id0_in_gl | id0_notin_gl].
+      inversion HupdateEnv; subst. clear HupdateEnv.
+      rewrite lookupGVMap_notin; auto.
+      rewrite lookupGVMap_updateGVMap_in; auto. 
+
+      inversion HupdateEnv; subst. clear HupdateEnv.
+      rewrite lookupGVMap_updateAddGVMap_eq; auto.
+Qed.
+
+Lemma lookupGVMap_updateGVMap_neq : forall m id0 id1 gv0,
+  id1 <> id0 ->
+  lookupGVMap m id1 = lookupGVMap (updateGVMap m id0 gv0) id1.
+Proof.
+  induction m; intros; simpl; auto.
+    destruct a.
+      destruct (@eq_dec id (@EqDec_eq_of_EqDec id EqDec_atom) id1 id0); subst; simpl; auto.
+        contradict H; auto.
+        destruct (@eq_dec id (@EqDec_eq_of_EqDec id EqDec_atom) id1 i0); subst; simpl; auto.
+          destruct (@eq_dec id (@EqDec_eq_of_EqDec id EqDec_atom) id0 i0); subst; simpl; auto.
+            contradict H; auto.
+            destruct (@eq_dec id (@EqDec_eq_of_EqDec id EqDec_atom) i0 i0); subst; simpl; auto.
+              contradict n1; auto.
+          destruct (@eq_dec id (@EqDec_eq_of_EqDec id EqDec_atom) id0 i0); subst; simpl; auto.
+            destruct (@eq_dec id (@EqDec_eq_of_EqDec id EqDec_atom) id1 i0); subst; simpl; auto.
+              contradict n; auto.
+            destruct (@eq_dec id (@EqDec_eq_of_EqDec id EqDec_atom) id1 i0); subst; simpl; auto.
+              contradict n0; auto.
+Qed.   
+
+Lemma lookupGVMap_updateAddGVMap_neq : forall m id0 id1 gv0,
+  id1 <> id0 ->
+  lookupGVMap m id1 = lookupGVMap (updateAddGVMap m id0 gv0) id1.
+Proof.
+  induction m; intros; simpl; auto.
+    destruct (id1==id0); subst; auto.
+      contradict H; auto.
+
+    destruct a.
+      destruct (@eq_dec id (@EqDec_eq_of_EqDec id EqDec_atom) id1 id0); subst; simpl; auto.
+        contradict H; auto.
+        destruct (@eq_dec id (@EqDec_eq_of_EqDec id EqDec_atom) id1 i0); subst; simpl; auto.
+          destruct (@eq_dec id (@EqDec_eq_of_EqDec id EqDec_atom) id0 i0); subst; simpl; auto.
+            contradict H; auto.
+            destruct (@eq_dec id (@EqDec_eq_of_EqDec id EqDec_atom) i0 i0); subst; simpl; auto.
+              contradict n1; auto.
+          destruct (@eq_dec id (@EqDec_eq_of_EqDec id EqDec_atom) id0 i0); subst; simpl; auto.
+            destruct (@eq_dec id (@EqDec_eq_of_EqDec id EqDec_atom) id1 i0); subst; simpl; auto.
+              contradict n; auto.
+            destruct (@eq_dec id (@EqDec_eq_of_EqDec id EqDec_atom) id1 i0); subst; simpl; auto.
+              contradict n0; auto.
+Qed.   
+
+Lemma lookupEnv_updateEnv_neq : forall id0 id1 lc gl gv0 lc' gl',
+  updateEnv lc gl id0 gv0 = (lc', gl') ->
+  id1 <> id0 ->
+  lookupEnv id1 lc gl = lookupEnv id1 lc' gl'.
+Proof.
+  intros id0 id1 lc gl ogv0 lc' gl' HupdateEnv id1_isnt_id0.
+  unfold updateEnv in HupdateEnv.
+  unfold lookupEnv.
+  destruct (@AtomSetProperties.In_dec id0 (dom lc)) as [id0_in_lc | id0_notin_lc].
+    inversion HupdateEnv; subst. clear HupdateEnv.
+    rewrite <- lookupGVMap_updateGVMap_neq; auto.
+
+    destruct (@AtomSetProperties.In_dec id0 (dom gl)) as [id0_in_gl | id0_notin_gl].
+      inversion HupdateEnv; subst. clear HupdateEnv.
+      rewrite <- lookupGVMap_updateGVMap_neq; auto.
+    
+      inversion HupdateEnv; subst. clear HupdateEnv.
+      rewrite <- lookupGVMap_updateAddGVMap_neq; auto.
+Qed. 
+
+
+Lemma lookupGVMap__indom : forall m id0 gv,
+  lookupGVMap m id0 = Some gv ->
+  id0 `in` dom m.
+Proof.
+  induction m; intros.
+    simpl in H. inversion H.
+
+    simpl in H. destruct a. 
+    destruct (id0==i0); subst; simpl; auto.
+      apply IHm in H; auto.
+Qed.  
+
+Lemma lookupEnv__indom : forall id0 lc gl gv,
+  lookupEnv id0 lc gl = Some gv ->
+  id0 `in` dom lc `union` dom gl.
+Proof.
+  intros id0 lc gl gv H.
+  unfold lookupEnv in H.
+  remember (lookupGVMap lc id0) as ogv.
+  destruct ogv.
+    symmetry in Heqogv.
+    apply lookupGVMap__indom in Heqogv; auto.
+
+    apply lookupGVMap__indom in H; auto.
+Qed.
+
+(**************************************)
+(** Convert const to GV with storesize, and look up GV from operands. *)
+
+Fixpoint _const2GV (TD:layouts) (c:const) : option (GenericValue*typ) := 
+match c with
+| const_int sz n => Some (nat2GV TD sz n, typ_int sz)
+| const_undef t =>  do gv <- undef2GV TD t; Some (gv, t)
+| const_null t =>   Some (ptr2GV TD null, t)
+| const_arr lc => 
+         fold_left 
+         (fun ogvt ogvt0 =>
+          match (ogvt, ogvt0) return option (GenericValue*typ) with
+          | (Some (gv, t), Some (gv0,t0)) =>
+             match (getTypeAllocSize TD t0) with
+             | Some sz0 => Some ((gv++gv0)++muninits (sz0 - length gv0), t0)
+             | None => None 
+             end
+          | _ => None
+          end
+         )
+         (Coq.Lists.List.map (_const2GV TD) lc)
+         (Some (nil, typ_int 0))
+| const_struct lc =>
+         match (fold_left 
+         (fun ogvtl ogvt0 =>
+          match (ogvtl, ogvt0) with
+          | (Some (gv, t, struct_al), Some (gv0,t0)) =>
+             match (getABITypeAlignment TD t0, getTypeAllocSize TD t0) with
+             | (Some sub_al, Some sub_sz) => 
+               match (le_lt_dec sub_al struct_al) with
+               | left _ (* struct_al <= sub_al *) =>
+                 Some (
+                  (gv++
+                  (muninits (sub_al - length gv0))++
+                  gv0++
+                  (muninits (sub_sz - length gv0)),
+                  t0),
+                  sub_al
+                 )
+               | right _ (* sub_al < struct_al *) =>
+                 Some (
+                  (gv++
+                  (muninits (sub_al - length gv0))++
+                  gv0++
+                  (muninits (sub_sz - length gv0)),
+                  t0),
+                  struct_al
+                 )
+               end
+             | _ => None 
+             end
+         | _ => None
+         end)
+         (Coq.Lists.List.map (_const2GV TD) lc)
+         (Some ((nil, typ_int 0), 0))) with
+         | None => None
+         | Some ((gv, t), al) => 
+           match (length gv) with
+           | 0 => Some (muninits al, t)
+           | _ => Some (gv++muninits (al-length gv), t)
+           end
+         end
+end.
+
+Definition const2GV (TD:layouts) (c:const) : option GenericValue :=
+match (_const2GV TD c) with
+| None => None
+| Some (gv, t) => Some gv
+end.
+
+Definition getOperandValue (TD:layouts) (v:value) (locals:GVMap) (globals:GVMap) : option GenericValue := 
+match v with
+| value_id id => lookupEnv id locals globals
+| value_const c => (const2GV TD c)
+end.
+
+Definition getOperandInt (TD:layouts) (sz:nat) (v:value) (locals:GVMap) (globals:GVMap) : option nat := 
+match (getOperandValue TD v locals globals) with
+| Some gi => (GV2nat TD sz gi)
+| None => None
+end.
+
+Definition isOperandUndef (TD:layouts) (t:typ) (v:value) (locals:GVMap) (globals:GVMap) : Prop  := 
+match (getOperandValue TD v locals globals) with
+| Some gi => isGVUndef TD t gi
+| None => False
+end.
+
+Definition getOperandPtr (TD:layouts) (v:value) (locals:GVMap) (globals:GVMap) : option mptr := 
+match (getOperandValue TD v locals globals) with
+| Some gi => GV2ptr TD (getPointerSize TD) gi
+| None => None
+end.
+
+Definition getOperandPtrInBits (TD:layouts) (s:sz) (v:value) (locals:GVMap) (globals:GVMap) : option mptr := 
+match (getOperandValue TD v locals globals) with
+| Some gi => GV2ptr TD s gi
+| None => None
+end.
+
+(**************************************)
+(* conversion between different lists *)
+
+Fixpoint params2OpGVs (TD:layouts) (lp:list_param) (locals:GVMap) (globals:GVMap) : list (option GenericValue):=
+match lp with
+| nil => nil
+| (_, v)::lp' => getOperandValue TD v locals globals::params2OpGVs TD lp' locals globals
+end.
+
+Fixpoint opGVs2GVs (lg:list (option GenericValue)) : list GenericValue :=
+match lg with
+| nil => nil
+| (Some g)::lg' => g::opGVs2GVs lg'
+| _::lg' => opGVs2GVs lg'
+end.
+
+Definition params2GVs (TD:layouts) (lp:list_param) (locals:GVMap) (globals:GVMap) := 
+  opGVs2GVs (params2OpGVs TD lp locals globals).
+
+Fixpoint intValues2Nats (TD:layouts) (lv:list value) (locals:GVMap) (globals:GVMap) : option (list nat):=
+match lv with
+| nil => Some nil
+| v::lv' => 
+  match (getOperandValue TD v locals globals) with
+  | Some GV => 
+    match (GV2nat TD 32 GV) with
+    | Some n =>
+      match (intValues2Nats TD lv' locals globals) with
+      | Some ns => Some (n::ns)
+      | None => None
+      end
+    | None => None
+    end
+  | None => None
+  end
+end.
+
+Fixpoint intConsts2Nats (TD:layouts) (lv:list const) : option (list nat):=
+match lv with
+| nil => Some nil
+| const_int 32 n::lv' => 
+  match (GV2nat TD 32 (nat2GV TD 32 n)) with
+  | Some n =>
+    match (intConsts2Nats TD lv') with
+    | Some ns => Some (n::ns)
+    | None => None
+    end
+  | None => None
+  end
+| _ => None
+end.
+
+Fixpoint GVs2Nats (TD:layouts) (lgv:list GenericValue) (locals:GVMap) (globals:GVMap) : option (list nat):=
+match lgv with
+| nil => Some nil
+| gv::lgv' => 
+    match (GV2nat TD 32 gv) with
+    | Some n =>
+      match (GVs2Nats TD lgv' locals globals) with
+      | Some ns => Some (n::ns)
+      | None => None
+      end
+    | None => None
+    end
+end.
+
+(**************************************)
+(* helping functions *)
+
+Fixpoint _initializeFrameValues (la:list_arg) (lg:list GenericValue) (locals:GVMap) : GVMap :=
+match (la, lg) with
+| ((_, id)::la', g::lg') => updateAddGVMap (_initializeFrameValues la' lg' locals) id g
+| _ => locals
+end.
+
+Definition initLocals (la:list_arg) (lg:list GenericValue): GVMap := 
+_initializeFrameValues la lg nil.
+
+Definition getEntryBlock (fd:fdef) : option block :=
+match fd with
+| fdef_intro _ (b::_) => Some b
+| _ => None
+end.
+
+Definition getEntryCmds (b:block) : list_cmd :=
+match b with
+| block_intro _ _ lc _ => lc
+end.
+
+(* FIXME : bounds check *)
+Definition extractGenericValue (TD:list layout)(t:typ) (gv : GenericValue) (cidxs : list const) : option GenericValue :=
+match (intConsts2Nats TD cidxs) with
+| None => None 
+| Some idxs =>
+  match (mgetoffset TD t idxs) with
+  | Some o => mget TD gv o t
+  | None => None
+  end
+end.
+
+Definition insertGenericValue (TD:list layout) (t:typ) (gv:GenericValue)
+  (cidxs:list const) (t0:typ) (gv0:GenericValue) : option GenericValue :=
+match (intConsts2Nats TD cidxs) with
+| None => None 
+| Some idxs =>
+  match (mgetoffset TD t idxs) with
+  | Some o => mset TD gv o t0 gv0
+  | None => None
+  end
+end.
+
+Definition GEP (TD:layouts) (locals globals:GVMap) (t:typ) (ma:mptr) (vidxs:list value) (inbounds:bool) : option mptr :=
+match (intValues2Nats TD vidxs locals globals) with
+| None => None 
+| Some idxs => mgep TD t ma idxs
+end.
+
+Definition mbop (TD:layouts) (op:bop) (bsz:sz) (gv1 gv2:mvalue) : option mvalue :=
+match op with
+| bop_add => 
+  match (GV2nat TD bsz gv1, GV2nat TD bsz gv2) with
+  | (Some i1, Some i2) => Some (nat2mvalue TD bsz (i1+i2))
+  | _ => None
+  end
+| _ => None
+end.
+
+Definition BOP (TD:layouts) (lc gl:GVMap) (op:bop) (bsz:sz) (v1 v2:value) : option mvalue :=
+match (getOperandValue TD v1 lc gl, getOperandValue TD v2 lc gl) with
+| (Some gv1, Some gv2) => mbop TD op bsz gv1 gv2
+| _ => None
+end
+.
+
+Definition mcast (TD:layouts) (op:castop) (t1:typ) (gv1:mvalue) (t2:typ) : option mvalue :=
+match op with
+| castop_inttoptr => 
+  match (t1, t2) with
+  | (typ_int sz1, typ_pointer _) => 
+    match (GV2ptr TD sz1 gv1) with
+    | Some mp1 => Some (ptr2GV TD mp1)
+    | None => None
+    end
+  | _ => None
+  end
+| castop_ptrtoint =>
+  match (t1, t2) with
+  | (typ_pointer _, typ_int sz2) => 
+    match (GV2ptr TD (getPointerSize TD) gv1) with
+    | Some mp1 => Some (mptr2mvalue TD mp1 sz2)
+    | None => None
+    end
+  | _ => None
+  end
+| castop_bitcase => Some gv1
+end.
+
+Definition CAST (TD:layouts) (lc gl:GVMap) (op:castop) (t1:typ) (v1:value) (t2:typ) : option mvalue :=
+match (getOperandValue TD v1 lc gl) with
+| (Some gv1) => mcast TD op t1 gv1 t2
+| _ => None
+end
+.
+
+Definition mext (TD:layouts) (op:extop) (t1:typ) (gv1:mvalue) (t2:typ) : option mvalue :=
+match op with
+| extop_z => 
+  match (t1, t2) with
+  | (typ_int sz1, typ_int sz2) => Some gv1
+  | _ => None
+  end
+| extop_s => 
+  match (t1, t2) with
+  | (typ_int sz1, typ_int sz2) => Some gv1
+  | _ => None
+  end
+end.
+
+Definition EXT (TD:layouts) (lc gl:GVMap) (op:extop) (t1:typ) (v1:value) (t2:typ) : option mvalue :=
+match (getOperandValue TD v1 lc gl) with
+| (Some gv1) => mext TD op t1 gv1 t2
+| _ => None
+end
+.
+
+Definition micmp (TD:layouts) (c:cond) (t:typ) (gv1 gv2:mvalue) : option mvalue :=
+match c with
+| cond_eq =>
+  match t with
+  | typ_int sz => None
+  | typ_pointer _ => None
+  | _ => None
+  end
+| cond_ne => None
+| cond_ugt => None
+| cond_uge => None
+| cond_ult => None
+| cond_ule => None
+| cond_sgt => None
+| cond_sge => None
+| cond_slt => None
+| cond_sle => None
+end.
+
+Definition ICMP (TD:layouts) (lc gl:GVMap) (c:cond) (t:typ) (v1 v2:value) : option mvalue :=
+match (getOperandValue TD v1 lc gl, getOperandValue TD v2 lc gl) with
+| (Some gv1, Some gv2) => micmp TD c t gv1 gv2
+| _ => None
+end.
+
+Lemma BOP_inversion : forall TD lc gl b s v1 v2 gv,
+  BOP TD lc gl b s v1 v2 = Some gv ->
+  exists gv1, exists gv2,
+    getOperandValue TD v1 lc gl = Some gv1 /\
+    getOperandValue TD v2 lc gl = Some gv2 /\
+    mbop TD b s gv1 gv2 = Some gv.
+Proof.
+  intros TD lc gl b s v1 v2 gv HBOP.
+  unfold BOP in HBOP.
+  remember (getOperandValue TD v1 lc gl) as ogv1.
+  destruct ogv1; try solve [inversion HBOP].
+    remember (getOperandValue TD v2 lc gl) as ogv2.
+    destruct ogv2; try solve [inversion HBOP].
+      remember (mbop TD b s g g0) as R.
+      destruct R; inversion HBOP; subst.
+        exists g. exists g0. auto.
+Qed.
+
+Lemma getOperandPtr_inversion : forall TD lc gl v mptr,
+  getOperandPtr TD v lc gl = Some mptr ->
+  exists gv,
+    getOperandValue TD v lc gl = Some gv /\
+    GV2ptr TD (getPointerSize TD) gv = Some mptr.
+Proof.
+  intros TD lc gl v mptr HgetOperandPtr.
+  unfold getOperandPtr in HgetOperandPtr.
+  remember (getOperandValue TD v lc gl) as ogv.
+  destruct ogv; try solve [inversion HgetOperandPtr].
+    exists g. auto.
+Qed.
+
+Lemma getOperandInt_inversion : forall TD sz lc gl v n,
+  getOperandInt TD sz v lc gl = Some n ->
+  exists gv,
+    getOperandValue TD v lc gl = Some gv /\
+    GV2nat TD sz gv = Some n.
+Proof.
+  intros TD sz0 lc gl v mptr HgetOperandInt.
+  unfold getOperandInt in HgetOperandInt.
+  remember (getOperandValue TD v lc gl) as ogv.
+  destruct ogv; try solve [inversion HgetOperandInt].
+    exists g. auto.
+Qed.
+
+Lemma CAST_inversion : forall TD lc gl op t1 v1 t2 gv,
+  CAST TD lc gl op t1 v1 t2 = Some gv ->
+  exists gv1,
+    getOperandValue TD v1 lc gl = Some gv1 /\
+    mcast TD op t1 gv1 t2 = Some gv.
+Proof.
+  intros TD lc gl op t1 v1 t2 gv HCAST.
+  unfold CAST in HCAST.
+  remember (getOperandValue TD v1 lc gl) as ogv1.
+  destruct ogv1; try solve [inversion HCAST].
+    remember (mcast TD op t1 g t2) as R.
+    destruct R; inversion HCAST; subst.
+      exists g. auto.
+Qed.
+
+Lemma EXT_inversion : forall TD lc gl op t1 v1 t2 gv,
+  EXT TD lc gl op t1 v1 t2 = Some gv ->
+  exists gv1,
+    getOperandValue TD v1 lc gl = Some gv1 /\
+    mext TD op t1 gv1 t2 = Some gv.
+Proof.
+  intros TD lc gl op t1 v1 t2 gv HEXT.
+  unfold EXT in HEXT.
+  remember (getOperandValue TD v1 lc gl) as ogv1.
+  destruct ogv1; try solve [inversion HEXT].
+    remember (mext TD op t1 g t2) as R.
+    destruct R; inversion HEXT; subst.
+      exists g. auto.
+Qed.
+
+Lemma ICMP_inversion : forall TD lc gl cond t v1 v2 gv,
+  ICMP TD lc gl cond t v1 v2 = Some gv ->
+  exists gv1, exists gv2,
+    getOperandValue TD v1 lc gl = Some gv1 /\
+    getOperandValue TD v2 lc gl = Some gv2 /\
+    micmp TD cond t gv1 gv2 = Some gv.
+Proof.
+  intros TD lc gl cond0 t v1 v2 gv HICMP.
+  unfold ICMP in HICMP.
+  remember (getOperandValue TD v1 lc gl) as ogv1.
+  destruct ogv1; try solve [inversion HICMP].
+    remember (getOperandValue TD v2 lc gl) as ogv2.
+    destruct ogv2; try solve [inversion HICMP].
+      remember (micmp TD cond0 t g g0) as R.
+      destruct R; inversion HICMP; subst.
+        exists g. exists g0. auto.
+Qed.
